@prefix : <https://w3id.org/omega-x/EUMEDMeteringOntology/> .
@prefix cc: <http://creativecommons.org/ns#> .
@prefix dc: <http://purl.org/dc/elements/1.1/> .
@prefix un: <https://qudt.org/vocab/unit#> .
@prefix vs: <http://www.w3.org/2003/06/sw-vocab-status/ns#> .
@prefix cur: <https://www.iso.org/iso-4217-currency-codes#> .
@prefix eme: <https://w3id.org/omega-x/EUMEDMeteringOntology#> .
@prefix msg: <http://langdale.com.au/2005/Message#> .
@prefix owl: <http://www.w3.org/2002/07/owl#> .
@prefix rdf: <http://www.w3.org/1999/02/22-rdf-syntax-ns#> .
@prefix xml: <http://www.w3.org/XML/1998/namespace> .
@prefix xsd: <http://www.w3.org/2001/XMLSchema#> .
@prefix foaf: <http://xmlns.com/foaf/0.1/> .
@prefix rdfs: <http://www.w3.org/2000/01/rdf-schema#> .
@prefix skos: <http://www.w3.org/2004/02/skos/core#> .
@prefix time: <http://www.w3.org/2006/time#> .
@prefix vann: <http://purl.org/vocab/vann/> .
@prefix voaf: <http://purl.org/vocommons/voaf#> .
@prefix dcterms: <http://purl.org/dc/terms/> .
@base <https://w3id.org/omega-x/EUMEDMeteringOntology/> .

<https://w3id.org/omega-x/EUMEDMeteringOntology> rdf:type owl:Ontology ;
                                                  owl:versionIRI <https://w3id.org/omega-x/EUMEDMeteringOntology-1.0> ;
                                                  dcterms:contributor [a foaf:Person ; foaf:name "Bruno Traverson" ] ;
                                                  dcterms:contributor [a foaf:Person ; foaf:name "Henon M. Lamboro" ] ;                                                                                                  
                                                  dcterms:creator <https://w3id.org/omega-x> ;
                                                  dcterms:license <https://opensource.org/license/mit/> ;
                                                  dcterms:created "2023-10-03"^^xsd:date ;                                                
                                                  dcterms:issued "2024-05-06"^^xsd:date; 
                                                  dcterms:modified "2024-05-03"^^xsd:date ;
                                                  dcterms:rights "Copyright © Omega-X Consortium 2022-2025"@en ;
                                                  dcterms:source <https://w3id.org/omega-x/ReferenceResources/EUMEDMetering/eumedMetering.xsd>,
                                                                  <https://w3id.org/omega-x/ReferenceResources/EUMEDMetering/eumedMeteringDataType.xsd> ;
                                                  dcterms:title "EUMED Metering Ontology"@en ;
                                                  dcterms:description: "European Commission develops Implementing Acts (IAs) that further define data interoperability requirements and procedures as stated in Articles 20, 23 and 24 of the Electricity Directive (EU) 2019/944. The European Union has adopted a customized implementation of IEC 61968-9:2022 named the “EUMED (EUropean My Energy Data) Metering profile”."@en ;
                                                  vann:preferredNamespacePrefix "eme" ;
                                                  vann:preferredNamespaceUri <https://w3id.org/omega-x> ;
                                                  rdfs:label "EUMED Metering Ontology"@en ;
                                                  owl:versionInfo "v1.0" ;
                                                  skos:scopeNote """EME is an ontology for representing EUMED Metering profile. EME is based around six main classes or groups of classes: 
                                                   MeterReadingSet class: encapsulates a set of Meter Readings (container of measured values), Usage Points (points related to the measurements) and Reading Types (characterization of the kind of the measured values).
                                                   Meter Reading group: composed of MeterReading, Meter, Customer and IntervalBlock classes. MeterReading gives the period of measurement for a series related to a given UsagePoint. It may be further characterized by Meter (reference to the physical device) and Customer (reference to the category/kind). IntervalBlock allows reference to ReadingType and access to individual readings.
                                                  Interval Reading group: composed of IntervalReading and ReadingQuality classes. IntervalReading contains the measured value and the time interval or the timestamp of the measurement. It may be associated to several reading quality attributes.
                                                  Usage Point group: composed of UsagePoint and UsagePointLocation classes. UsagePoint identifies a logical or physical device related to the measurements optionally characterized by a location.
                                                   Reading Type class: gathers 16 technical parameters that permit to characterize the set of measured values composing a Meter Reading.
                                                  Name group: composed of Name, NameType and NameTypeAuthority classes. This is an optional way to identify Usage Points and Reading Types."""@en .

#---------------------------------------------------------------
#    Annotation properties
#--------------------------------------------------------------

dcterms:contributor rdf:type owl:AnnotationProperty .
dcterms:created rdf:type owl:AnnotationProperty .
dcterms:creator rdf:type owl:AnnotationProperty .
dcterms:issued rdf:type owl:AnnotationProperty .
dcterms:license rdf:type owl:AnnotationProperty .
dcterms:modified rdf:type owl:AnnotationProperty .
dcterms:right rdf:type owl:AnnotationProperty .
dcterms:source rdf:type owl:AnnotationProperty .
dcterms:title rdf:type owl:AnnotationProperty .
dcterms:description: rdf:type owl:AnnotationProperty .
vann:preferredNamespacePrefix rdf:type owl:AnnotationProperty .
vann:preferredNamespaceUri rdf:type owl:AnnotationProperty .
skos:scopeNote rdf:type owl:AnnotationProperty .


#----------------------------------------------------------------
#    Classes
#----------------------------------------------------------------

time:DateTimeInterval rdf:type owl:Class .

#-- AccumulationKind
eme:AccumulationKind rdf:type owl:Class ;
                     rdfs:subClassOf eme:Datatype ;
                     rdfs:comment "Kind of accumulation behaviour for read or measured values from individual end points."@en ;
                     rdfs:label "accumulation kind"@en .

#-- AggregateKind
eme:AggregateKind rdf:type owl:Class ;
                  rdfs:subClassOf eme:Datatype ;
                  rdfs:comment "Kind of aggregation for read or measured values from multiple end points."@en ;
                  rdfs:label "aggregate kind"@en .

#-- CommodityKind
eme:CommodityKind rdf:type owl:Class ;
                  rdfs:subClassOf eme:Datatype ;
                  rdfs:comment "Kind of commodity being measured."@en ;
                  rdfs:label "commodity kind"@en .

#-- Currency
eme:Currency rdf:type owl:Class ;
             rdfs:subClassOf eme:Datatype ;
             rdfs:comment "Monetary currencies.  ISO 4217 standard including 3-character currency code."@en ;
             rdfs:label "currency"@en .


#-- Customer
eme:Customer rdf:type owl:Class ;
             rdfs:subClassOf eme:Entity ;
             rdfs:comment "Organisation receiving services from service supplier."@en ;
             rdfs:label "customer"@en .

#-- CustomerKind
eme:CustomerKind rdf:type owl:Class ;
                 rdfs:subClassOf eme:Datatype ;
                 rdfs:comment "Kind of customer."@en ;
                 rdfs:label "customer kind"@en .

#-- Datatype
eme:Datatype rdf:type owl:Class ;
             rdfs:comment "TBA"@en ;
             rdfs:label "datatype"@en .

#-- Entity
eme:Entity rdf:type owl:Class ;
           rdfs:comment "TBA"@en ;
           rdfs:label "entity"@en .

#-- FlowDirectionKind
eme:FlowDirectionKind rdf:type owl:Class ;
                      rdfs:subClassOf eme:Datatype ;
                      rdfs:comment "Kind of flow direction for reading or measured  values proper to some commodities such as, for example, energy, power, demand."@en ;
                      rdfs:label "flow direction kind"@en .

#-- IntervalBlock
eme:IntervalBlock rdf:type owl:Class ;
                  rdfs:subClassOf eme:Entity ;
                  rdfs:comment "Time sequence of readings of the same reading type. Contained interval readings may need conversion through the application of an offset and a scalar defined in associated pending."@en ;
                  rdfs:label "interval block"@en .

#-- IntervalReading
eme:IntervalReading rdf:type owl:Class ;
                    rdfs:subClassOf eme:Entity ,
                                    [ rdf:type owl:Restriction ;
                                      owl:onProperty eme:hasTimePeriod ;
                                      owl:qualifiedCardinality "1"^^xsd:nonNegativeInteger ;
                                      owl:onClass time:DateTimeInterval
                                    ] ;
                    rdfs:comment """Data captured at regular intervals of time. Interval data could be captured as incremental data, absolute data, or relative data. The source for the data is usually a tariff quantity or an engineering quantity. Data is typically captured in time-tagged, uniform, fixed-length intervals of 5 min, 10 min, 15 min, 30 min, or 60 min.
Note: Interval Data is sometimes also called \"Interval Data Readings\" (IDR)."""@en ;
                    rdfs:label "interval reading"@en .

#-- MacroPeriodKind
eme:MacroPeriodKind rdf:type owl:Class ;
                    rdfs:subClassOf eme:Datatype ;
                    rdfs:comment "Kind of macro period for calculations on read or measured values."@en ;
                    rdfs:label "macro period kind"@en .

#-- MeasurementKind
eme:MeasurementKind rdf:type owl:Class ;
                    rdfs:subClassOf eme:Datatype .


#-- MeasuringPeriodKind
eme:MeasuringPeriodKind rdf:type owl:Class ;
                        rdfs:subClassOf eme:Datatype ;
                        rdfs:comment "Kind of period for reading or measuring values"@en ;
                        rdfs:label "measuring period kind"@en .

#-- Meter
eme:Meter rdf:type owl:Class ;
          rdfs:subClassOf eme:Entity ;
          rdfs:comment "Physical asset that performs the metering role of the usage point. Used for measuring consumption and detection of events."@en ;
          rdfs:label "meter"@en .

#-- MeterReading
eme:MeterReading rdf:type owl:Class ;
                 rdfs:subClassOf eme:Entity ,
                                 [ rdf:type owl:Restriction ;
                                   owl:onProperty eme:hasValuesInterval ;
                                   owl:qualifiedCardinality "1"^^xsd:nonNegativeInteger ;
                                   owl:onClass time:DateTimeInterval
                                 ] ;
                 rdfs:comment "Set of values obtained from the meter."@en ;
                 rdfs:label "meter reading"@en .

#-- MeterReadingSet
eme:MeterReadingSet rdf:type owl:Class ;
                    rdfs:subClassOf eme:Entity ;
                    rdfs:comment """encapsulates a set of Meter Readings (container of measured
values), Usage Points (points related to the measurements) and Reading Types
(characterization of the kind of the measured values)."""@en ;
                    rdfs:label "meter reading set"@en .

#-- Name
eme:Name rdf:type owl:Class ;
         rdfs:subClassOf eme:Entity ;
         rdfs:comment "The Name class provides the means to define any number of human readable  names for an object. A name is not to be used for defining inter-object relationships. For inter-object relationships instead use the object identification 'mRID'."@en ;
         rdfs:label "name"@en .


#-- NameType
eme:NameType rdf:type owl:Class ;
             rdfs:subClassOf eme:Entity ;
             rdfs:comment """Type of name. Possible values for attribute 'name' are implementation dependent but standard profiles may specify types. An enterprise may have multiple IT systems each having its own local name for the same object, e.g. a planning system may have different names from an EMS. An object may also have different names within the same IT system, e.g. localName as defined in CIM version 14. The definition from CIM14 is:
The localName is a human readable name of the object. It is a free text name local to a node in a naming hierarchy similar to a file directory structure. A power system related naming hierarchy may be: Substation, VoltageLevel, Equipment etc. Children of the same parent in such a hierarchy have names that typically are unique among them."""@en ;
             rdfs:label "name type"@en .


#-- NameTypeAuthority
eme:NameTypeAuthority rdf:type owl:Class ;
                      rdfs:subClassOf eme:Entity ;
                      rdfs:comment "Authority responsible for creation and management of names of a given type; typically an organization or an enterprise system."@en ;
                      rdfs:label "name type authority"@en .


#-- PhaseCode
eme:PhaseCode rdf:type owl:Class ;
              rdfs:subClassOf eme:Datatype ;
              rdfs:comment """An unordered enumeration of phase identifiers.  Allows designation of phases for both transmission and distribution equipment, circuits and loads.   The enumeration, by itself, does not describe how the phases are connected together or connected to ground.  Ground is not explicitly denoted as a phase.
Residential and small commercial loads are often served from single-phase, or split-phase, secondary circuits. For the example of s12N, phases 1 and 2 refer to hot wires that are 180 degrees out of phase, while N refers to the neutral wire. Through single-phase transformer connections, these secondary circuits may be served from one or two of the primary phases A, B, and C. For three-phase loads, use the A, B, C phase codes instead of s12N.
The integer values are from IEC 61968-9 to support revenue metering applications."""@en ;
              rdfs:label "phase code"@en .

#-- ReadingQuality
eme:ReadingQuality rdf:type owl:Class ;
                   rdfs:subClassOf eme:Entity ;
                   rdfs:comment "Quality of a specific reading value or interval reading value. Note that more than one quality may be applicable to a given reading. Typically not used unless problems or unusual conditions occur (i.e., quality for each reading is assumed to be good unless stated otherwise in associated reading quality type). It can also be used with the corresponding reading quality type to indicate that the validation has been performed and succeeded."@en ;
                   rdfs:label "reading quality"@en .

#-- ReadingType
eme:ReadingType rdf:type owl:Class ;
                rdfs:subClassOf eme:Entity ;
                rdfs:comment "Detailed description for a type of a reading value. Values in attributes allow for the creation of recommended codes to be used for identifying reading value types as follows: <macroPeriod>.<aggregate>.<measuringPeriod>.<accumulation>.<flowDirection>.<commodity>.<measurementKind>.<interharmonic.numerator>.<interharmonic.denominator>.<argument.numerator>.<argument.denominator>.<tou>.<cpp>.<consumptionTier>.<phases>.<multiplier>.<unit>.<currency>."@en ;
                rdfs:label "reading type"@en .

#-- UnitMultiplier
eme:UnitMultiplier rdf:type owl:Class ;
                   rdfs:subClassOf eme:Datatype ;
                   rdfs:comment """The unit multipliers defined for the CIM.  When applied to unit symbols, the unit symbol is treated as a derived unit. Regardless of the contents of the unit symbol text, the unit symbol shall be treated as if it were a single-character unit symbol. Unit symbols should not contain multipliers, and it should be left to the multiplier to define the multiple for an entire data type. 

For example, if a unit symbol is \"m2Pers\" and the multiplier is \"k\", then the value is k(m**2/s), and the multiplier applies to the entire final value, not to any individual part of the value. This can be conceptualized by substituting a derived unit symbol for the unit type. If one imagines that the symbol \"Þ\" represents the derived unit \"m2Pers\", then applying the multiplier \"k\" can be conceptualized simply as \"kÞ\".

For example, the SI unit for mass is \"kg\" and not \"g\".  If the unit symbol is defined as \"kg\", then the multiplier is applied to \"kg\" as a whole and does not replace the \"k\" in front of the \"g\". In this case, the multiplier of \"m\" would be used with the unit symbol of \"kg\" to represent one gram.  As a text string, this violates the instructions in IEC 80000-1. However, because the unit symbol in CIM is treated as a derived unit instead of as an SI unit, it makes more sense to conceptualize the \"kg\" as if it were replaced by one of the proposed replacements for the SI mass symbol. If one imagines that the \"kg\" were replaced by a symbol \"Þ\", then it is easier to conceptualize the multiplier \"m\" as creating the proper unit \"mÞ\", and not the forbidden unit \"mkg\"."""@en ;
                   rdfs:label "unit multiplier"@en .

#-- UnitSymbol
eme:UnitSymbol rdf:type owl:Class ;
               rdfs:subClassOf eme:Datatype ;
               rdfs:comment """The derived units defined for usage in the CIM. In some cases, the derived unit is equal to an SI unit. Whenever possible, the standard derived symbol is used instead of the formula for the derived unit. For example, the unit symbol Farad is defined as \"F\" instead of \"CPerV\". In cases where a standard symbol does not exist for a derived unit, the formula for the unit is used as the unit symbol. For example, density does not have a standard symbol and so it is represented as \"kgPerm3\". With the exception of the \"kg\", which is an SI unit, the unit symbols do not contain multipliers and therefore represent the base derived unit to which a multiplier can be applied as a whole. 
Every unit symbol is treated as an unparseable text as if it were a single-letter symbol. The meaning of each unit symbol is defined by the accompanying descriptive text and not by the text contents of the unit symbol.
To allow the widest possible range of serializations without requiring special character handling, several substitutions are made which deviate from the format described in IEC 80000-1. The division symbol \"/\" is replaced by the letters \"Per\". Exponents are written in plain text after the unit as \"m3\" instead of being formatted as \"m\" with a superscript of 3  or introducing a symbol as in \"m^3\". The degree symbol \"°\" is replaced with the letters \"deg\". Any clarification of the meaning for a substitution is included in the description for the unit symbol.
Non-SI units are included in list of unit symbols to allow sources of data to be correctly labelled with their non-SI units (for example, a GPS sensor that is reporting numbers that represent feet instead of meters). This allows software to use the unit symbol information correctly convert and scale the raw data of those sources into SI-based units. 
The integer values are used for harmonization with IEC 61850."""@en ;
               rdfs:label "unit symbol"@en .

#-- UsagePoint
eme:UsagePoint rdf:type owl:Class ;
               rdfs:subClassOf eme:Entity ;
               rdfs:comment "Logical or physical point in the network to which readings or events may be attributed. Used at the place where a physical or virtual meter may be located; however, it is not required that a meter be present."@en ;
               rdfs:label "usage point"@en .

#-- UsagePointLocation
eme:UsagePointLocation rdf:type owl:Class ;
                       rdfs:subClassOf eme:Entity ;
                       rdfs:comment "Location of an individual usage point."@en ;
                       rdfs:label "usage point location"@en .




#--------------------------------------------------------------
#    Object Properties
#--------------------------------------------------------------


#-- appliesToIntervalReading
eme:appliesToIntervalReading rdf:type owl:ObjectProperty ;
                             owl:inverseOf eme:hasReadingQuality ;
                             rdfs:domain eme:ReadingQuality ;
                             rdfs:range eme:IntervalReading ;
                             rdfs:comment "Reading value to which this quality applies."@en ;
                             rdfs:label "applies to interval reading"@en .
                             

#-- hasAccumulation
eme:hasAccumulation rdf:type owl:ObjectProperty ;
                    rdfs:domain eme:ReadingType ;
                    rdfs:range eme:AccumulationKind ;
                    rdfs:comment "Accumulation behaviour of a reading over time, usually 'measuringPeriod', to be used with individual endpoints (as opposed to 'macroPeriod' and 'aggregate' that are used to describe aggregations of data from individual endpoints)."@en ;
                    rdfs:label "has accumulation"@en .

#-- hasAggregate
eme:hasAggregate rdf:type owl:ObjectProperty ;
                 rdfs:domain eme:ReadingType ;
                 rdfs:range eme:AggregateKind ;
                 rdfs:comment "Salient attribute of the reading data aggregated from individual endpoints. This is mainly used to define a mathematical operation carried out over 'macroPeriod', but may also be used to describe an attribute of the data when the 'macroPeriod' is not defined."@en ,
                              "has aggregate"@en .

#-- hasCommodity
eme:hasCommodity rdf:type owl:ObjectProperty ;
                 rdfs:domain eme:ReadingType ;
                 rdfs:range eme:CommodityKind ;
                 rdfs:comment "Commodity being measured."@en ;
                 rdfs:label "has commodity"@en .

#-- hasCurrency
eme:hasCurrency rdf:type owl:ObjectProperty ;
                rdfs:domain eme:ReadingType ;
                rdfs:range eme:Currency ;
                rdfs:comment "Metering-specific currency."@en ;
                rdfs:label "has currency"@en .

#-- hasFlowDirection
eme:hasFlowDirection rdf:type owl:ObjectProperty ;
                     rdfs:domain eme:ReadingType ;
                     rdfs:range eme:FlowDirectionKind ;
                     rdfs:comment "Flow direction for a reading where the direction of flow of the commodity is important (for electricity measurements this includes current, energy, power, and demand)."@en ;
                     rdfs:label "has flow direction" .

#-- hasKind
eme:hasKind rdf:type owl:ObjectProperty ;
            rdfs:domain eme:Customer ;
            rdfs:range eme:CustomerKind ;
            rdfs:comment "Kind of customer."@en ;
            rdfs:label "has kind"@en .

#-- hasMacroPeriod
eme:hasMacroPeriod rdf:type owl:ObjectProperty ;
                   rdfs:domain eme:ReadingType ;
                   rdfs:range eme:MacroPeriodKind ;
                   rdfs:comment "Time period of interest that reflects how the reading is viewed or captured over a long period of time."@en ;
                   rdfs:label "has macro period"@en .

#-- hasMeasurementKind
eme:hasMeasurementKind rdf:type owl:ObjectProperty ;
                       rdfs:domain eme:ReadingType ;
                       rdfs:range eme:MeasurementKind ;
                       rdfs:comment "Identifies \"what\" is being measured, as refinement of 'commodity'. When combined with 'unit', it provides detail to the unit of measure. For example, 'energy' with a unit of measure of 'kWh' indicates to the user that active energy is being measured, while with 'kVAh' or 'kVArh', it indicates apparent energy and reactive energy, respectively. 'power' can be combined in a similar way with various power units of measure: Distortion power ('distortionVoltAmperes') with 'kVA' is different from 'power' with 'kVA'."@en ;
                       rdfs:label "has measurement kind"@en .

#-- hasMeasuringPeriod
eme:hasMeasuringPeriod rdf:type owl:ObjectProperty ;
                       rdfs:domain eme:ReadingType ;
                       rdfs:range eme:MeasuringPeriodKind ;
                       rdfs:comment """Time attribute inherent or fundamental to the reading value (as opposed to 'macroPeriod' that supplies an \"adjective\" to describe aspects of a time period with regard to the measurement). It refers to the way the value was originally measured and not to the frequency at which it is reported or presented. For example, an hourly interval of consumption data would have value 'hourly' as an attribute. However in the case of an hourly sampled voltage value, the meterReadings schema would carry the 'hourly' interval size information.
It is common for meters to report demand in a form that is measured over the course of a portion of an hour, while enterprise applications however commonly assume the demand (in kW or kVAr) normalised to 1 hour. The system that receives readings directly from the meter therefore shall perform this transformation before publishing readings for use by the other enterprise systems. The scalar used is chosen based on the block size (not any sub-interval size)."""@en ,
                                    "has measuring period"@en .

#-- hasMeterReading
eme:hasMeterReading rdf:type owl:ObjectProperty ;
                    owl:inverseOf eme:isRelatedToUsagePoint ;
                    rdfs:domain eme:UsagePoint ;
                    rdfs:range eme:MeterReading ;
                    rdfs:comment "All meter readings obtained from this usage point."@en ;
                    rdfs:label "has meter readings"@en .

#-- hasMultiplier
eme:hasMultiplier rdf:type owl:ObjectProperty ;
                  rdfs:domain eme:ReadingType ;
                  rdfs:range eme:UnitMultiplier ;
                  rdfs:comment "Metering-specific multiplier."@en ;
                  rdfs:label "has multiplier"@en .

#-- hasNameAsReadingType
eme:hasNameAsReadingType rdf:type owl:ObjectProperty ;
                         rdfs:domain eme:ReadingType ;
                         rdfs:range eme:Name ;
                         rdfs:comment "All names of this reading type."@en ;
                         rdfs:label "has name as reading type"@en .

#-- hasNameAsUsagePoint
eme:hasNameAsUsagePoint rdf:type owl:ObjectProperty ;
                        rdfs:domain eme:UsagePoint ;
                        rdfs:range eme:Name ;
                        rdfs:comment "All names of this usage point."@en ;
                        rdfs:label "has name as usage point"@en .

#-- hasNameType
eme:hasNameType rdf:type owl:ObjectProperty ;
                rdfs:domain eme:Name ;
                rdfs:range eme:NameType ;
                rdfs:comment "Type of this name."@en ;
                rdfs:label "has name type"@en .

#-- hasNameTypeAuthority
eme:hasNameTypeAuthority rdf:type owl:ObjectProperty ;
                         rdfs:domain eme:NameType ;
                         rdfs:range eme:NameTypeAuthority ;
                         rdfs:comment "Authority responsible for managing names of this type."@en ;
                         rdfs:label "has name type authority"@en .

#-- hasPhases
eme:hasPhases rdf:type owl:ObjectProperty ;
              rdfs:domain eme:ReadingType ;
              rdfs:range eme:PhaseCode ;
              rdfs:comment "Metering-specific phase code."@en ;
              rdfs:label "has phases"@en .

#-- hasReadingQuality
eme:hasReadingQuality rdf:type owl:ObjectProperty ;
                      rdfs:domain eme:IntervalReading ;
                      rdfs:range eme:ReadingQuality ;
                      rdfs:comment "has reading qualities"@en ,
                                   "All qualities of this reading." .

#-- hasReadingType
eme:hasReadingType rdf:type owl:ObjectProperty ;
                   owl:inverseOf eme:isUsedByIntervalBlock ;
                   rdfs:domain eme:IntervalBlock ;
                   rdfs:range eme:ReadingType ;
                   rdfs:comment "Type information for interval reading values contained in this block."@en ,
                                "has reading type"@en .

#-- hasTimePeriod
eme:hasTimePeriod rdf:type owl:ObjectProperty ;
                  rdfs:domain eme:IntervalReading ;
                  rdfs:range time:DateTimeInterval ;
                  rdfs:comment "Start and end of the period for those readings whose type has a time attribute such as 'billing', seasonal' or 'forTheSpecifiedPeriod'."@en ;
                  rdfs:label "time period"@en .

#-- hasUnit
eme:hasUnit rdf:type owl:ObjectProperty ;
            rdfs:domain eme:ReadingType ;
            rdfs:range eme:UnitSymbol ;
            rdfs:comment "Metering-specific unit."@en ;
            rdfs:label "has unit"@en .

#-- hasUsagePointLocation
eme:hasUsagePointLocation rdf:type owl:ObjectProperty ;
                          rdfs:domain eme:UsagePoint ;
                          rdfs:range eme:UsagePointLocation ;
                          rdfs:comment "All usage points at this location."@en ;
                          rdfs:label "locates usage point"@en .

#-- hasValuesInterval
eme:hasValuesInterval rdf:type owl:ObjectProperty ;
                      rdfs:domain eme:MeterReading ;
                      rdfs:range time:DateTimeInterval ;
                      rdfs:comment "Date and time interval of the data items contained within this meter reading."@en ;
                      rdfs:label "values interval"@en .

#-- isComposedOfIntervalBlock
eme:isComposedOfIntervalBlock rdf:type owl:ObjectProperty ;
                              rdfs:domain eme:MeterReading ;
                              rdfs:range eme:IntervalBlock ;
                              rdfs:comment "All interval blocks contained in this meter reading."@en ;
                              rdfs:label "is composed of interval blocks"@en .

#-- isComposedOfIntervalReading
eme:isComposedOfIntervalReading rdf:type owl:ObjectProperty ;
                                owl:inverseOf eme:isPartofIntervalBlock ;
                                rdfs:domain eme:IntervalBlock ;
                                rdfs:range eme:IntervalReading ;
                                rdfs:comment "Interval reading contained in this block."@en ;
                                rdfs:label "is composed of interval readings"@en .

#-- isComposedOfMeterReading
eme:isComposedOfMeterReading rdf:type owl:ObjectProperty ;
                             owl:inverseOf eme:isMeterReadingAsPartOfMeterReadingSet ;
                             rdfs:domain eme:MeterReadingSet ;
                             rdfs:range eme:MeterReading ;
                             rdfs:comment "TBA"@en ;
                             rdfs:label "is composed of meter readings"@en .

#-- isComposedOfReadingType
eme:isComposedOfReadingType rdf:type owl:ObjectProperty ;
                            owl:inverseOf eme:isReadingTypeAsPartOfMeterReadingSet ;
                            rdfs:domain eme:MeterReadingSet ;
                            rdfs:range eme:ReadingType ;
                            rdfs:comment "TBA"@en ;
                            rdfs:label "is composed of reading types"@en .

#-- isComposedOfUsagePoint
eme:isComposedOfUsagePoint rdf:type owl:ObjectProperty ;
                           owl:inverseOf eme:isUsagePointAsPartOfMeterReadingSet ;
                           rdfs:domain eme:MeterReadingSet ;
                           rdfs:range eme:UsagePoint ;
                           rdfs:comment "TBA"@en ;
                           rdfs:label "is composed of usage points"@en .

#-- isLocatedAtUsagePointLocation
eme:isLocatedAtUsagePointLocation rdf:type owl:ObjectProperty ;
                                  rdfs:domain eme:UsagePoint ;
                                  rdfs:range eme:UsagePointLocation ;
                                  rdfs:comment "Location of this usage point."@en ;
                                  rdfs:label "usage point usage point location"@en .

#-- isMeterReadingAsPartOfMeterReadingSet
eme:isMeterReadingAsPartOfMeterReadingSet rdf:type owl:ObjectProperty ;
                                          rdfs:comment "TBA"@en ,
                                                       "is meter reading as part of meter reading set"@en .


#-- isOwnedbyCustomer
eme:isOwnedbyCustomer rdf:type owl:ObjectProperty ;
                      owl:inverseOf eme:ownsMeter ;
                      rdfs:domain eme:Meter ;
                      rdfs:range eme:Customer ;
                      rdfs:comment "Customer owning this end device."@en ;
                      rdfs:label "is owned by customer"@en .

#-- isPartofIntervalBlock
eme:isPartofIntervalBlock rdf:type owl:ObjectProperty ;
                          rdfs:domain eme:IntervalReading ;
                          rdfs:range eme:IntervalBlock ;
                          rdfs:comment "Interval block containing this interval reading."@en ;
                          rdfs:label "is part of interval block"@en .

#-- isProvidedByMeter
eme:isProvidedByMeter rdf:type owl:ObjectProperty ;
                      owl:inverseOf eme:providesMeterReading ;
                      rdfs:domain eme:MeterReading ;
                      rdfs:range eme:Meter ;
                      rdfs:comment "Meter providing this reading." ;
                      rdfs:label "is provided by meter" .

#-- isReadingTypeAsPartOfMeterReadingSet
eme:isReadingTypeAsPartOfMeterReadingSet rdf:type owl:ObjectProperty ;
                                         rdfs:comment "TBA"@en ;
                                         rdfs:label "is reading type as part of meter reading set"@en .


#-- isRelatedToUsagePoint
eme:isRelatedToUsagePoint rdf:type owl:ObjectProperty ;
                          rdfs:domain eme:MeterReading ;
                          rdfs:range eme:UsagePoint ;
                          rdfs:comment "Usage point from which this meter reading (set of values) has been obtained."@en ;
                          rdfs:label "is obtained by usage point"@en .

#-- isUsagePointAsPartOfMeterReadingSet
eme:isUsagePointAsPartOfMeterReadingSet rdf:type owl:ObjectProperty ;
                                        rdfs:label "is usage point as part of meter reading set"@en .


#-- isUsedByIntervalBlock
eme:isUsedByIntervalBlock rdf:type owl:ObjectProperty ;
                          rdfs:domain eme:ReadingType ;
                          rdfs:range eme:IntervalBlock ;
                          rdfs:comment "All blocks containing interval reading values with this type information."@en ;
                          rdfs:label "is used by interval block"@en .

#-- ownsMeter
eme:ownsMeter rdf:type owl:ObjectProperty ;
              rdfs:domain eme:Customer ;
              rdfs:range eme:Meter ;
              rdfs:comment "All end devices of this customer."@en ;
              rdfs:label "owns meter"@en .

#-- providesMeterReading
eme:providesMeterReading rdf:type owl:ObjectProperty ;
                         rdfs:domain eme:Meter ;
                         rdfs:range eme:MeterReading ;
                         rdfs:comment "All meter readings provided by this meter."@en ;
                         rdfs:label "provides meter readings"@en .


#--------------------------------------------------------------
#    Datatypes
#--------------------------------------------------------------

xsd:date rdf:type rdfs:Datatype .


#--------------------------------------------------------------
#    Data properties
#--------------------------------------------------------------

#-- comment
eme:comment rdf:type owl:DatatypeProperty ;
            rdfs:domain eme:ReadingQuality ;
            rdfs:range xsd:string ;
            rdfs:comment "Elaboration on the quality code."@en ;
            rdfs:label "comment"@en .

#-- consumptionTier
eme:consumptionTier rdf:type owl:DatatypeProperty ;
                    rdfs:domain eme:ReadingType ;
                    rdfs:range xsd:integer ;
                    rdfs:comment """In case of common flat-rate pricing for power, in which all purchases are at a given rate, 'consumptionTier'=0. Otherwise, the value indicates the consumption tier, which can be used in conjunction with TOU or CPP pricing.
Consumption tier pricing refers to the method of billing in which a certain \"block\" of energy is purchased/sold at one price, after which the next block of energy is purchased at another price, and so on, all throughout a defined period. At the start of the defined period, consumption is initially zero, and any usage is measured against the first consumption tier ('consumptionTier'=1). If this block of energy is consumed before the end of the period, energy consumption moves to be reconed against the second consumption tier ('consumptionTier'=2), and so on. At the end of the defined period, the consumption accumulator is reset, and usage within the 'consumptionTier'=1 restarts."""@en ;
                    rdfs:label "consumption tier"@en .

#-- cpp
eme:cpp rdf:type owl:DatatypeProperty ;
        rdfs:domain eme:ReadingType ;
        rdfs:range xsd:integer ;
        rdfs:comment "Critical peak period (CPP) bucket the reading value is attributed to. Value 0 means not applicable. Even though CPP is usually considered a specialised form of time of use 'tou', this attribute is defined explicitly for flexibility."@en ;
        rdfs:label "cpp"@en .

#-- geoInfoReference
eme:geoInfoReference rdf:type owl:DatatypeProperty ;
                     rdfs:domain eme:UsagePointLocation ;
                     rdfs:range xsd:string ;
                     rdfs:comment "(if applicable) Reference to geographical information source, often external to the utility."@en ;
                     rdfs:label "geo info reference"@en .

#-- installCode
eme:installCode rdf:type owl:DatatypeProperty ;
                rdfs:domain eme:Meter ;
                rdfs:range xsd:string ;
                rdfs:comment "Installation code."@en ;
                rdfs:label "install code"@en .

#-- mRID
eme:mRID rdf:type owl:DatatypeProperty ;
         rdfs:domain [ rdf:type owl:Class ;
                       owl:unionOf ( eme:IntervalReading
                                     eme:MeterReading
                                     eme:ReadingType
                                     eme:UsagePoint
                                   )
                     ] ;
         rdfs:range xsd:string ;
         rdfs:comment "Master resource identifier issued by a model authority. The mRID is unique within an exchange context. Global uniqueness is easily achieved by using a UUID, as specified in RFC 4122, for the mRID. The use of UUID is strongly recommended. For CIMXML data files in RDF syntax conforming to IEC 61970-552, the mRID is mapped to rdf:ID or rdf:about attributes that identify CIM object elements."@en ;
         rdfs:label "mRID"@en .

#-- name
eme:name rdf:type owl:DatatypeProperty ;
         rdfs:domain [ rdf:type owl:Class ;
                       owl:unionOf ( eme:IntervalReading
                                     eme:MeterReading
                                     eme:Name
                                     eme:NameType
                                     eme:NameTypeAuthority
                                   )
                     ] ;
         rdfs:range xsd:string ;
         rdfs:comment "The name is any free human readable and possibly non unique text naming the object."@en ;
         rdfs:isDefinedBy <http://iec.ch/TC57/EUMED-Metering#EUMED_Metering_ENTITIES/name> ;
         rdfs:label "name"@en .


#-- rationalNumber
eme:rationalNumber rdf:type owl:DatatypeProperty ;
                   rdfs:domain eme:ReadingType ;
                   rdfs:range [ rdf:type rdfs:Datatype ;
                                owl:oneOf [ rdf:type rdf:List ;
                                            rdf:first "denominator" ;
                                            rdf:rest [ rdf:type rdf:List ;
                                                       rdf:first "numerator" ;
                                                       rdf:rest rdf:nil
                                                     ]
                                          ]
                              ] ;
                   rdfs:comment "Rational number = 'numerator' over 'denominator'."@en ;
                   rdfs:label "rational number"@en .

#-- readingInterharmonic
eme:readingInterharmonic rdf:type owl:DatatypeProperty ;
                         rdfs:domain eme:ReadingType ;
                         rdfs:range [ rdf:type rdfs:Datatype ;
                                      owl:oneOf [ rdf:type rdf:List ;
                                                  rdf:first "denominator" ;
                                                  rdf:rest [ rdf:type rdf:List ;
                                                             rdf:first "numerator" ;
                                                             rdf:rest rdf:nil
                                                           ]
                                                ]
                                    ] ;
                         rdfs:comment "Interharmonics are represented as a rational number 'numerator' over 'denominator', and harmonics are represented using the same mechanism and identified by 'denominator'=1."@en ;
                         rdfs:label "reading interharmonic"@en .

#-- timeStamp
eme:timeStamp rdf:type owl:DatatypeProperty ;
              rdfs:domain eme:IntervalReading ;
              rdfs:range xsd:dateTime ;
              rdfs:comment "The time when the value was last updated."@en ;
              rdfs:label "time stamp"@en .

#-- tou
eme:tou rdf:type owl:DatatypeProperty ;
        rdfs:domain eme:ReadingType ;
        rdfs:range xsd:integer ;
        rdfs:comment "Time of use (TOU) bucket the reading value is attributed to. A value of “0” means that TOU is not applicable to this measurement."@en ;
        rdfs:label "tou"@en .

#-- value
eme:value rdf:type owl:DatatypeProperty ;
          rdfs:domain eme:IntervalReading ;
          rdfs:comment "Value of interval reading."@en ;
          rdfs:label "value"@en .

#--------------------------------------------------------------
#    Individuals
#--------------------------------------------------------------

#-- A
eme:A rdf:type owl:NamedIndividual ,
               eme:PhaseCode ;
      rdfs:comment "Phase A."@en ;
      rdfs:label "A"@en .


#-- A2
eme:A2 rdf:type owl:NamedIndividual ,
                eme:UnitSymbol ;
       rdfs:comment "Amperes squared A." ;
       rdfs:label "A2"@en .


#-- A2h
eme:A2h rdf:type owl:NamedIndividual ,
                 eme:UnitSymbol ;
        rdfs:comment "Amperesquared hour amperesquared hour." ;
        rdfs:label "A2h"@en .


#-- A2s
eme:A2s rdf:type owl:NamedIndividual ,
                 eme:UnitSymbol ;
        rdfs:comment "Ampere squared time in square amperes As." ;
        rdfs:label "A2s"@en .


#-- AB
eme:AB rdf:type owl:NamedIndividual ,
                eme:PhaseCode ;
       rdfs:comment "Phases A and B."@en .


#-- ABC
eme:ABC rdf:type owl:NamedIndividual ,
                 eme:PhaseCode ;
        rdfs:comment "Phases A, B, and C."@en .


#-- ABCN
eme:ABCN rdf:type owl:NamedIndividual ,
                  eme:PhaseCode ;
         rdfs:comment "Phases A, B, C, and N."@en .


#-- ABN
eme:ABN rdf:type owl:NamedIndividual ,
                 eme:PhaseCode ;
        rdfs:comment "Phases A, B, and neutral."@en .


#-- AC
eme:AC rdf:type owl:NamedIndividual ,
                eme:PhaseCode ;
       rdfs:comment "Phases A and C."@en .


#-- ACN
eme:ACN rdf:type owl:NamedIndividual ,
                 eme:PhaseCode ;
        rdfs:comment "Phases A, C and neutral."@en .


#-- AED
eme:AED rdf:type owl:NamedIndividual ,
                 eme:Currency ;
        rdfs:comment "United Arab Emirates dirham." ;
        rdfs:label "AED"@en .


#-- AFN
eme:AFN rdf:type owl:NamedIndividual ,
                 eme:Currency ;
        rdfs:comment "Afghan afghani." ;
        rdfs:label "AFN"@en .


#-- ALL
eme:ALL rdf:type owl:NamedIndividual ,
                 eme:Currency ;
        rdfs:comment "Albanian lek." ;
        rdfs:label "ALL"@en .


#-- AMD
eme:AMD rdf:type owl:NamedIndividual ,
                 eme:Currency ;
        rdfs:comment "Armenian dram." ;
        rdfs:label "AMD"@en .


#-- AN
eme:AN rdf:type owl:NamedIndividual ,
                eme:PhaseCode ;
       rdfs:comment "Phases A and neutral."@en .


#-- ANG
eme:ANG rdf:type owl:NamedIndividual ,
                 eme:Currency ;
        rdfs:comment "Netherlands Antillean guilder." ;
        rdfs:label "ANG"@en .


#-- AOA
eme:AOA rdf:type owl:NamedIndividual ,
                 eme:Currency ;
        rdfs:comment "Angolan kwanza." ;
        rdfs:label "AOA"@en .


#-- APerA
eme:APerA rdf:type owl:NamedIndividual ,
                   eme:UnitSymbol ;
          rdfs:comment "Current ratio of amperages.   Note Users may need to supply a prefix such as m to show rates such as mAA." ;
          rdfs:label "APerA"@en .


#-- APerm
eme:APerm rdf:type owl:NamedIndividual ,
                   eme:UnitSymbol ;
          rdfs:comment "Am magnetic field strength amperes per metre." ;
          rdfs:label "APerm"@en .


#-- ARS
eme:ARS rdf:type owl:NamedIndividual ,
                 eme:Currency ;
        rdfs:comment "Argentine peso." ;
        rdfs:label "ARS"@en .


#-- AUD
eme:AUD rdf:type owl:NamedIndividual ,
                 eme:Currency ;
        rdfs:comment "Australian dollar." ;
        rdfs:label "AUD"@en .


#-- AWG
eme:AWG rdf:type owl:NamedIndividual ,
                 eme:Currency ;
        rdfs:comment "Aruban florin." ;
        rdfs:label "AWG"@en .


#-- AZN
eme:AZN rdf:type owl:NamedIndividual ,
                 eme:Currency ;
        rdfs:comment "Azerbaijani manat." ;
        rdfs:label "AZN"@en .


#-- Ah
eme:Ah rdf:type owl:NamedIndividual ,
                eme:UnitSymbol ;
       rdfs:comment "Amperehours amperehours." ;
       rdfs:label "Ah"@en .


#-- As
eme:As rdf:type owl:NamedIndividual ,
                eme:UnitSymbol ;
       rdfs:comment "Ampere seconds As." ;
       rdfs:label "As"@en .


#-- Aunit
eme:Aunit rdf:type owl:NamedIndividual ,
                   eme:UnitSymbol ;
          rdfs:comment "Current in amperes."@en ;
          rdfs:label "A"@en .


#-- B
eme:B rdf:type owl:NamedIndividual ,
               eme:PhaseCode ;
      rdfs:comment "Phase B."@en .


#-- BAM
eme:BAM rdf:type owl:NamedIndividual ,
                 eme:Currency ;
        rdfs:comment "Bosnia and Herzegovina convertible mark." ;
        rdfs:label "BAM"@en .


#-- BBD
eme:BBD rdf:type owl:NamedIndividual ,
                 eme:Currency ;
        rdfs:comment "Barbados dollar." ;
        rdfs:label "BBD"@en .


#-- BC
eme:BC rdf:type owl:NamedIndividual ,
                eme:PhaseCode ;
       rdfs:comment "Phases B and C." .


#-- BCN
eme:BCN rdf:type owl:NamedIndividual ,
                 eme:PhaseCode ;
        rdfs:comment "Phases B, C, and neutral."@en .


#-- BDT
eme:BDT rdf:type owl:NamedIndividual ,
                 eme:Currency ;
        rdfs:comment "Bangladeshi taka." ;
        rdfs:label "BDT"@en .


#-- BGN
eme:BGN rdf:type owl:NamedIndividual ,
                 eme:Currency ;
        rdfs:comment "Bulgarian lev." ;
        rdfs:label "BGN"@en .


#-- BHD
eme:BHD rdf:type owl:NamedIndividual ,
                 eme:Currency ;
        rdfs:comment "Bahraini dinar." ;
        rdfs:label "BHD"@en .


#-- BIF
eme:BIF rdf:type owl:NamedIndividual ,
                 eme:Currency ;
        rdfs:comment "Burundian franc." ;
        rdfs:label "BIF"@en .


#-- BMD
eme:BMD rdf:type owl:NamedIndividual ,
                 eme:Currency ;
        rdfs:comment "Bermudian dollar customarily known as Bermuda dollar." ;
        rdfs:label "BMD"@en .


#-- BN
eme:BN rdf:type owl:NamedIndividual ,
                eme:PhaseCode ;
       rdfs:comment "Phases B and neutral."@en .


#-- BND
eme:BND rdf:type owl:NamedIndividual ,
                 eme:Currency ;
        rdfs:comment "Brunei dollar." ;
        rdfs:label "BND"@en .


#-- BOB
eme:BOB rdf:type owl:NamedIndividual ,
                 eme:Currency ;
        rdfs:comment "Boliviano." ;
        rdfs:label "BOB"@en .


#-- BOV
eme:BOV rdf:type owl:NamedIndividual ,
                 eme:Currency ;
        rdfs:comment "Bolivian Mvdol funds code." ;
        rdfs:label "BOV"@en .


#-- BRL
eme:BRL rdf:type owl:NamedIndividual ,
                 eme:Currency ;
        rdfs:comment "Brazilian real." ;
        rdfs:label "BRL"@en .


#-- BSD
eme:BSD rdf:type owl:NamedIndividual ,
                 eme:Currency ;
        rdfs:comment "Bahamian dollar." ;
        rdfs:label "BSD"@en .


#-- BTN
eme:BTN rdf:type owl:NamedIndividual ,
                 eme:Currency ;
        rdfs:comment "Bhutanese ngultrum." ;
        rdfs:label "BTN"@en .


#-- BWP
eme:BWP rdf:type owl:NamedIndividual ,
                 eme:Currency ;
        rdfs:comment "Botswana pula." ;
        rdfs:label "BWP"@en .


#-- BYR
eme:BYR rdf:type owl:NamedIndividual ,
                 eme:Currency ;
        rdfs:comment "Belarusian ruble." ;
        rdfs:label "BYR"@en .


#-- BZD
eme:BZD rdf:type owl:NamedIndividual ,
                 eme:Currency ;
        rdfs:comment "Belize dollar." ;
        rdfs:label "BZD"@en .


#-- Bq
eme:Bq rdf:type owl:NamedIndividual ,
                eme:UnitSymbol ;
       rdfs:comment "Radioactivity in becquerels 1s." ;
       rdfs:label "Bq"@en .


#-- Btu
eme:Btu rdf:type owl:NamedIndividual ,
                 eme:UnitSymbol ;
        rdfs:comment "Energy British Thermal Units." ;
        rdfs:label "Btu"@en .


#-- C
eme:C rdf:type owl:NamedIndividual ,
               eme:PhaseCode ;
      rdfs:comment "Phase C."@en ;
      rdfs:label "C"@en .


#-- CAD
eme:CAD rdf:type owl:NamedIndividual ,
                 eme:Currency ;
        rdfs:comment "Canadian dollar." ;
        rdfs:label "CAD"@en .


#-- CDF
eme:CDF rdf:type owl:NamedIndividual ,
                 eme:Currency ;
        rdfs:comment "Congolese franc." ;
        rdfs:label "CDF"@en .


#-- CHF
eme:CHF rdf:type owl:NamedIndividual ,
                 eme:Currency ;
        rdfs:comment "Swiss franc." ;
        rdfs:label "CHF"@en .


#-- CLF
eme:CLF rdf:type owl:NamedIndividual ,
                 eme:Currency ;
        rdfs:comment "Unidad de Fomento funds code Chile." ;
        rdfs:label "CLF"@en .


#-- CLP
eme:CLP rdf:type owl:NamedIndividual ,
                 eme:Currency ;
        rdfs:comment "Chilean peso." ;
        rdfs:label "CLP"@en .


#-- CN
eme:CN rdf:type owl:NamedIndividual ,
                eme:PhaseCode ;
       rdfs:comment "Phases C and neutral."@en .


#-- CNY
eme:CNY rdf:type owl:NamedIndividual ,
                 eme:Currency ;
        rdfs:comment "Chinese yuan." ;
        rdfs:label "CNY"@en .


#-- COP
eme:COP rdf:type owl:NamedIndividual ,
                 eme:Currency ;
        rdfs:comment "Colombian peso." ;
        rdfs:label "COP"@en .


#-- COU
eme:COU rdf:type owl:NamedIndividual ,
                 eme:Currency ;
        rdfs:comment "Unidad de Valor Real." ;
        rdfs:label "COU"@en .


#-- CPerkg
eme:CPerkg rdf:type owl:NamedIndividual ,
                    eme:UnitSymbol ;
           rdfs:comment "Exposure x rays coulombs per kilogram." ;
           rdfs:label "CPerkg"@en .


#-- CPerm2
eme:CPerm2 rdf:type owl:NamedIndividual ,
                    eme:UnitSymbol ;
           rdfs:comment "Surface charge density coulombs per square metre." ;
           rdfs:label "CPerm2"@en .


#-- CPerm3
eme:CPerm3 rdf:type owl:NamedIndividual ,
                    eme:UnitSymbol ;
           rdfs:comment "Electric charge density coulombs per cubic metre." ;
           rdfs:label "CPerm3"@en .


#-- CRC
eme:CRC rdf:type owl:NamedIndividual ,
                 eme:Currency ;
        rdfs:comment "Costa Rican colon." ;
        rdfs:label "CRC"@en .


#-- CUC
eme:CUC rdf:type owl:NamedIndividual ,
                 eme:Currency ;
        rdfs:comment "Cuban convertible peso." ;
        rdfs:label "CUC"@en .


#-- CUP
eme:CUP rdf:type owl:NamedIndividual ,
                 eme:Currency ;
        rdfs:comment "Cuban peso." ;
        rdfs:label "CUP"@en .


#-- CVE
eme:CVE rdf:type owl:NamedIndividual ,
                 eme:Currency ;
        rdfs:comment "Cape Verde escudo." ;
        rdfs:label "CVE"@en .


#-- CZK
eme:CZK rdf:type owl:NamedIndividual ,
                 eme:Currency ;
        rdfs:comment "Czech koruna." ;
        rdfs:label "CZK"@en .


#-- Cunit
eme:Cunit rdf:type owl:NamedIndividual ,
                   eme:UnitSymbol ;
          rdfs:comment "Electric charge in coulombs As."@en ;
          rdfs:label "C"@en .


#-- DJF
eme:DJF rdf:type owl:NamedIndividual ,
                 eme:Currency ;
        rdfs:comment "Djiboutian franc." ;
        rdfs:label "DJF"@en .


#-- DKK
eme:DKK rdf:type owl:NamedIndividual ,
                 eme:Currency ;
        rdfs:comment "Danish krone." ;
        rdfs:label "DKK"@en .


#-- DOP
eme:DOP rdf:type owl:NamedIndividual ,
                 eme:Currency ;
        rdfs:comment "Dominican peso." ;
        rdfs:label "DOP"@en .


#-- DZD
eme:DZD rdf:type owl:NamedIndividual ,
                 eme:Currency ;
        rdfs:comment "Algerian dinar." ;
        rdfs:label "DZD"@en .


#-- E
eme:E rdf:type owl:NamedIndividual ,
               eme:UnitMultiplier ;
      rdfs:comment "Exa 1018." ;
      rdfs:label "E"@en .


#-- EEK
eme:EEK rdf:type owl:NamedIndividual ,
                 eme:Currency ;
        rdfs:comment "Estonian kroon." ;
        rdfs:label "EEK"@en .


#-- EGP
eme:EGP rdf:type owl:NamedIndividual ,
                 eme:Currency ;
        rdfs:comment "Egyptian pound." ;
        rdfs:label "EGP"@en .


#-- ERN
eme:ERN rdf:type owl:NamedIndividual ,
                 eme:Currency ;
        rdfs:comment "Eritrean nakfa." ;
        rdfs:label "ERN"@en .


#-- ETB
eme:ETB rdf:type owl:NamedIndividual ,
                 eme:Currency ;
        rdfs:comment "Ethiopian birr." ;
        rdfs:label "ETB"@en .


#-- EUR
eme:EUR rdf:type owl:NamedIndividual ,
                 eme:Currency ;
        rdfs:comment "Euro." ;
        rdfs:label "EUR"@en .


#-- F
eme:F rdf:type owl:NamedIndividual ,
               eme:UnitSymbol ;
      rdfs:comment "Electric capacitance in farads CV." ;
      rdfs:label "F"@en .


#-- FJD
eme:FJD rdf:type owl:NamedIndividual ,
                 eme:Currency ;
        rdfs:comment "Fiji dollar." ;
        rdfs:label "FJD"@en .


#-- FKP
eme:FKP rdf:type owl:NamedIndividual ,
                 eme:Currency ;
        rdfs:comment "Falkland Islands pound." ;
        rdfs:label "FKP"@en .


#-- FPerm
eme:FPerm rdf:type owl:NamedIndividual ,
                   eme:UnitSymbol ;
          rdfs:comment "Permittivity farads per metre." ;
          rdfs:label "FPerm"@en .


#-- G
eme:G rdf:type owl:NamedIndividual ,
               eme:UnitMultiplier ,
               eme:UnitSymbol ;
      rdfs:comment "Giga 109." ,
                   "Magnetic flux density gausses 1 G  104 T." ;
      rdfs:label "G"@en .


#-- GBP
eme:GBP rdf:type owl:NamedIndividual ,
                 eme:Currency ;
        rdfs:comment "Pound sterling." ;
        rdfs:label "GBP"@en .


#-- GEL
eme:GEL rdf:type owl:NamedIndividual ,
                 eme:Currency ;
        rdfs:comment "Georgian lari." ;
        rdfs:label "GEL"@en .


#-- GHS
eme:GHS rdf:type owl:NamedIndividual ,
                 eme:Currency ;
        rdfs:comment "Ghanaian cedi." ;
        rdfs:label "GHS"@en .


#-- GIP
eme:GIP rdf:type owl:NamedIndividual ,
                 eme:Currency ;
        rdfs:comment "Gibraltar pound." ;
        rdfs:label "GIP"@en .


#-- GMD
eme:GMD rdf:type owl:NamedIndividual ,
                 eme:Currency ;
        rdfs:comment "Gambian dalasi." ;
        rdfs:label "GMD"@en .


#-- GNF
eme:GNF rdf:type owl:NamedIndividual ,
                 eme:Currency ;
        rdfs:comment "Guinean franc." ;
        rdfs:label "GNF"@en .


#-- GTQ
eme:GTQ rdf:type owl:NamedIndividual ,
                 eme:Currency ;
        rdfs:comment "Guatemalan quetzal." ;
        rdfs:label "GTQ"@en .


#-- GYD
eme:GYD rdf:type owl:NamedIndividual ,
                 eme:Currency ;
        rdfs:comment "Guyanese dollar." ;
        rdfs:label "GYD"@en .


#-- Gy
eme:Gy rdf:type owl:NamedIndividual ,
                eme:UnitSymbol ;
       rdfs:comment "Absorbed dose in grays Jkg." ;
       rdfs:label "Gy"@en .


#-- GyPers
eme:GyPers rdf:type owl:NamedIndividual ,
                    eme:UnitSymbol ;
           rdfs:comment "Absorbed dose rate grays per second." ;
           rdfs:label "GyPers"@en .


#-- H
eme:H rdf:type owl:NamedIndividual ,
               eme:UnitSymbol ;
      rdfs:comment "Electric inductance in henrys WbA." ;
      rdfs:label "H"@en .


#-- HKD
eme:HKD rdf:type owl:NamedIndividual ,
                 eme:Currency ;
        rdfs:comment "Hong Kong dollar." ;
        rdfs:label "HKD"@en .


#-- HNL
eme:HNL rdf:type owl:NamedIndividual ,
                 eme:Currency ;
        rdfs:comment "Honduran lempira." ;
        rdfs:label "HNL"@en .


#-- HPerm
eme:HPerm rdf:type owl:NamedIndividual ,
                   eme:UnitSymbol ;
          rdfs:comment "Permeability henrys per metre." ;
          rdfs:label "HPerm"@en .


#-- HRK
eme:HRK rdf:type owl:NamedIndividual ,
                 eme:Currency ;
        rdfs:comment "Croatian kuna." ;
        rdfs:label "HRK"@en .


#-- HTG
eme:HTG rdf:type owl:NamedIndividual ,
                 eme:Currency ;
        rdfs:comment "Haitian gourde." ;
        rdfs:label "HTG"@en .


#-- HUF
eme:HUF rdf:type owl:NamedIndividual ,
                 eme:Currency ;
        rdfs:comment "Hungarian forint." ;
        rdfs:label "HUF"@en .


#-- Hz
eme:Hz rdf:type owl:NamedIndividual ,
                eme:UnitSymbol ;
       rdfs:comment "Frequency in hertz 1s." ;
       rdfs:label "Hz"@en .


#-- HzPerHz
eme:HzPerHz rdf:type owl:NamedIndividual ,
                     eme:UnitSymbol ;
            rdfs:comment "Frequency rate of frequency change.   Note Users may need to supply a prefix such as m to show rates such as mHzHz." ;
            rdfs:label "HzPerHz"@en .


#-- HzPers
eme:HzPers rdf:type owl:NamedIndividual ,
                    eme:UnitSymbol ;
           rdfs:comment "Rate of change of frequency in hertz per second." ;
           rdfs:label "HzPers"@en .


#-- IDR
eme:IDR rdf:type owl:NamedIndividual ,
                 eme:Currency ;
        rdfs:comment "Indonesian rupiah." ;
        rdfs:label "IDR"@en .


#-- ILS
eme:ILS rdf:type owl:NamedIndividual ,
                 eme:Currency ;
        rdfs:comment "Israeli new sheqel." ;
        rdfs:label "ILS"@en .


#-- INR
eme:INR rdf:type owl:NamedIndividual ,
                 eme:Currency ;
        rdfs:comment "Indian rupee." ;
        rdfs:label "INR"@en .


#-- IQD
eme:IQD rdf:type owl:NamedIndividual ,
                 eme:Currency ;
        rdfs:comment "Iraqi dinar." ;
        rdfs:label "IQD"@en .


#-- IRR
eme:IRR rdf:type owl:NamedIndividual ,
                 eme:Currency ;
        rdfs:comment "Iranian rial." ;
        rdfs:label "IRR"@en .


#-- ISK
eme:ISK rdf:type owl:NamedIndividual ,
                 eme:Currency ;
        rdfs:comment "Icelandic krna." ;
        rdfs:label "ISK"@en .


#-- J
eme:J rdf:type owl:NamedIndividual ,
               eme:UnitSymbol ;
      rdfs:comment "Energy in joules Nm  CV  Ws." ;
      rdfs:label "J"@en .


#-- JMD
eme:JMD rdf:type owl:NamedIndividual ,
                 eme:Currency ;
        rdfs:comment "Jamaican dollar." ;
        rdfs:label "JMD"@en .


#-- JOD
eme:JOD rdf:type owl:NamedIndividual ,
                 eme:Currency ;
        rdfs:comment "Jordanian dinar." ;
        rdfs:label "JOD"@en .


#-- JPY
eme:JPY rdf:type owl:NamedIndividual ,
                 eme:Currency ;
        rdfs:comment "Japanese yen." ;
        rdfs:label "JPY"@en .


#-- JPerK
eme:JPerK rdf:type owl:NamedIndividual ,
                   eme:UnitSymbol ;
          rdfs:comment "Heat capacity in jouleskelvin." ;
          rdfs:label "JPerK"@en .


#-- JPerkg
eme:JPerkg rdf:type owl:NamedIndividual ,
                    eme:UnitSymbol ;
           rdfs:comment "Specific energy Joules  kg." ;
           rdfs:label "JPerkg"@en .


#-- JPerkgK
eme:JPerkgK rdf:type owl:NamedIndividual ,
                     eme:UnitSymbol ;
            rdfs:comment "Specific heat capacity specific entropy joules per kilogram Kelvin." ;
            rdfs:label "JPerkgK"@en .


#-- JPerm2
eme:JPerm2 rdf:type owl:NamedIndividual ,
                    eme:UnitSymbol ;
           rdfs:comment "Insulation energy density joules per square metre or watt second per square metre." ;
           rdfs:label "JPerm2"@en .


#-- JPerm3
eme:JPerm3 rdf:type owl:NamedIndividual ,
                    eme:UnitSymbol ;
           rdfs:comment "Energy density joules per cubic metre." ;
           rdfs:label "JPerm3"@en .


#-- JPermol
eme:JPermol rdf:type owl:NamedIndividual ,
                     eme:UnitSymbol ;
            rdfs:comment "Molar energy joules per mole." ;
            rdfs:label "JPermol"@en .


#-- JPermolK
eme:JPermolK rdf:type owl:NamedIndividual ,
                      eme:UnitSymbol ;
             rdfs:comment "Molar entropy molar heat capacity joules per mole kelvin." ;
             rdfs:label "JPermolK"@en .


#-- JPers
eme:JPers rdf:type owl:NamedIndividual ,
                   eme:UnitSymbol ;
          rdfs:comment "Energy rate in joules per second Js." ;
          rdfs:label "JPers"@en .


#-- K
eme:K rdf:type owl:NamedIndividual ,
               eme:UnitSymbol ;
      rdfs:comment "Temperature in kelvins." ;
      rdfs:label "K"@en .


#-- KES
eme:KES rdf:type owl:NamedIndividual ,
                 eme:Currency ;
        rdfs:comment "Kenyan shilling." ;
        rdfs:label "KES"@en .


#-- KGS
eme:KGS rdf:type owl:NamedIndividual ,
                 eme:Currency ;
        rdfs:comment "Kyrgyzstani som." ;
        rdfs:label "KGS"@en .


#-- KHR
eme:KHR rdf:type owl:NamedIndividual ,
                 eme:Currency ;
        rdfs:comment "Cambodian riel." ;
        rdfs:label "KHR"@en .


#-- KMF
eme:KMF rdf:type owl:NamedIndividual ,
                 eme:Currency ;
        rdfs:comment "Comoro franc." ;
        rdfs:label "KMF"@en .


#-- KPW
eme:KPW rdf:type owl:NamedIndividual ,
                 eme:Currency ;
        rdfs:comment "North Korean won." ;
        rdfs:label "KPW"@en .


#-- KPers
eme:KPers rdf:type owl:NamedIndividual ,
                   eme:UnitSymbol ;
          rdfs:comment "Temperature change rate in kelvins per second." ;
          rdfs:label "KPers"@en .


#-- KRW
eme:KRW rdf:type owl:NamedIndividual ,
                 eme:Currency ;
        rdfs:comment "South Korean won." ;
        rdfs:label "KRW"@en .


#-- KWD
eme:KWD rdf:type owl:NamedIndividual ,
                 eme:Currency ;
        rdfs:comment "Kuwaiti dinar." ;
        rdfs:label "KWD"@en .


#-- KYD
eme:KYD rdf:type owl:NamedIndividual ,
                 eme:Currency ;
        rdfs:comment "Cayman Islands dollar." ;
        rdfs:label "KYD"@en .


#-- KZT
eme:KZT rdf:type owl:NamedIndividual ,
                 eme:Currency ;
        rdfs:comment "Kazakhstani tenge." ;
        rdfs:label "KZT"@en .


#-- LAK
eme:LAK rdf:type owl:NamedIndividual ,
                 eme:Currency ;
        rdfs:comment "Lao kip." ;
        rdfs:label "LAK"@en .


#-- LBP
eme:LBP rdf:type owl:NamedIndividual ,
                 eme:Currency ;
        rdfs:comment "Lebanese pound." ;
        rdfs:label "LBP"@en .


#-- LKR
eme:LKR rdf:type owl:NamedIndividual ,
                 eme:Currency ;
        rdfs:comment "Sri Lanka rupee." ;
        rdfs:label "LKR"@en .


#-- LRD
eme:LRD rdf:type owl:NamedIndividual ,
                 eme:Currency ;
        rdfs:comment "Liberian dollar." ;
        rdfs:label "LRD"@en .


#-- LSL
eme:LSL rdf:type owl:NamedIndividual ,
                 eme:Currency ;
        rdfs:comment "Lesotho loti." ;
        rdfs:label "LSL"@en .


#-- LTL
eme:LTL rdf:type owl:NamedIndividual ,
                 eme:Currency ;
        rdfs:comment "Lithuanian litas." ;
        rdfs:label "LTL"@en .


#-- LVL
eme:LVL rdf:type owl:NamedIndividual ,
                 eme:Currency ;
        rdfs:comment "Latvian lats." ;
        rdfs:label "LVL"@en .


#-- LYD
eme:LYD rdf:type owl:NamedIndividual ,
                 eme:Currency ;
        rdfs:comment "Libyan dinar." ;
        rdfs:label "LYD"@en .


#-- M
eme:M rdf:type owl:NamedIndividual ,
               eme:UnitMultiplier ,
               eme:UnitSymbol ;
      rdfs:comment "Length nautical miles 1 M  1852 m." ,
                   "Mega 106." ;
      rdfs:label "M"@en .


#-- MAD
eme:MAD rdf:type owl:NamedIndividual ,
                 eme:Currency ;
        rdfs:comment "Moroccan dirham." ;
        rdfs:label "MAD"@en .


#-- MDL
eme:MDL rdf:type owl:NamedIndividual ,
                 eme:Currency ;
        rdfs:comment "Moldovan leu." ;
        rdfs:label "MDL"@en .


#-- MGA
eme:MGA rdf:type owl:NamedIndividual ,
                 eme:Currency ;
        rdfs:comment "Malagasy ariary." ;
        rdfs:label "MGA"@en .


#-- MKD
eme:MKD rdf:type owl:NamedIndividual ,
                 eme:Currency ;
        rdfs:comment "Macedonian denar." ;
        rdfs:label "MKD"@en .


#-- MMK
eme:MMK rdf:type owl:NamedIndividual ,
                 eme:Currency ;
        rdfs:comment "Myanma kyat." ;
        rdfs:label "MMK"@en .


#-- MNT
eme:MNT rdf:type owl:NamedIndividual ,
                 eme:Currency ;
        rdfs:comment "Mongolian tugrik." ;
        rdfs:label "MNT"@en .


#-- MOP
eme:MOP rdf:type owl:NamedIndividual ,
                 eme:Currency ;
        rdfs:comment "Macanese pataca." ;
        rdfs:label "MOP"@en .


#-- MRO
eme:MRO rdf:type owl:NamedIndividual ,
                 eme:Currency ;
        rdfs:comment "Mauritanian ouguiya." ;
        rdfs:label "MRO"@en .


#-- MUR
eme:MUR rdf:type owl:NamedIndividual ,
                 eme:Currency ;
        rdfs:comment "Mauritian rupee." ;
        rdfs:label "MUR"@en .


#-- MVR
eme:MVR rdf:type owl:NamedIndividual ,
                 eme:Currency ;
        rdfs:comment "Maldivian rufiyaa." ;
        rdfs:label "MVR"@en .


#-- MWK
eme:MWK rdf:type owl:NamedIndividual ,
                 eme:Currency ;
        rdfs:comment "Malawian kwacha." ;
        rdfs:label "MWK"@en .


#-- MXN
eme:MXN rdf:type owl:NamedIndividual ,
                 eme:Currency ;
        rdfs:comment "Mexican peso." ;
        rdfs:label "MXN"@en .


#-- MYR
eme:MYR rdf:type owl:NamedIndividual ,
                 eme:Currency ;
        rdfs:comment "Malaysian ringgit." ;
        rdfs:label "MYR"@en .


#-- MZN
eme:MZN rdf:type owl:NamedIndividual ,
                 eme:Currency ;
        rdfs:comment "Mozambican metical." ;
        rdfs:label "MZN"@en .


#-- Mx
eme:Mx rdf:type owl:NamedIndividual ,
                eme:UnitSymbol ;
       rdfs:comment "Magnetic flux maxwells 1 Mx  108 Wb." ;
       rdfs:label "Mx"@en .


#-- N
eme:N rdf:type owl:NamedIndividual ,
               eme:PhaseCode ,
               eme:UnitSymbol ;
      rdfs:comment "Neutral phase."@en ,
                   "Force in newtons kgms." ;
      rdfs:label "N"@en .


#-- NAD
eme:NAD rdf:type owl:NamedIndividual ,
                 eme:Currency ;
        rdfs:comment "Namibian dollar." ;
        rdfs:label "NAD"@en .


#-- NGN
eme:NGN rdf:type owl:NamedIndividual ,
                 eme:Currency ;
        rdfs:comment "Nigerian naira." ;
        rdfs:label "NGN"@en .


#-- NIO
eme:NIO rdf:type owl:NamedIndividual ,
                 eme:Currency ;
        rdfs:comment "Cordoba oro." ;
        rdfs:label "NIO"@en .


#-- NOK
eme:NOK rdf:type owl:NamedIndividual ,
                 eme:Currency ;
        rdfs:comment "Norwegian krone." ;
        rdfs:label "NOK"@en .


#-- NPR
eme:NPR rdf:type owl:NamedIndividual ,
                 eme:Currency ;
        rdfs:comment "Nepalese rupee." ;
        rdfs:label "NPR"@en .


#-- NPerm
eme:NPerm rdf:type owl:NamedIndividual ,
                   eme:UnitSymbol ;
          rdfs:comment "Surface tension newton per metre." ;
          rdfs:label "NPerm"@en .


#-- NZD
eme:NZD rdf:type owl:NamedIndividual ,
                 eme:Currency ;
        rdfs:comment "New Zealand dollar." ;
        rdfs:label "NZD"@en .


#-- Nm
eme:Nm rdf:type owl:NamedIndividual ,
                eme:UnitSymbol ;
       rdfs:comment "Moment of force newton metres." ;
       rdfs:label "Nm"@en .


#-- OMR
eme:OMR rdf:type owl:NamedIndividual ,
                 eme:Currency ;
        rdfs:comment "Omani rial." ;
        rdfs:label "OMR"@en .


#-- Oe
eme:Oe rdf:type owl:NamedIndividual ,
                eme:UnitSymbol ;
       rdfs:comment "Magnetic field in oersteds 1 Oe  1034p Am." ;
       rdfs:label "Oe"@en .


#-- P
eme:P rdf:type owl:NamedIndividual ,
               eme:UnitMultiplier ;
      rdfs:comment "Peta 1015." ;
      rdfs:label "P"@en .


#-- PAB
eme:PAB rdf:type owl:NamedIndividual ,
                 eme:Currency ;
        rdfs:comment "Panamanian balboa." ;
        rdfs:label "PAB"@en .


#-- PEN
eme:PEN rdf:type owl:NamedIndividual ,
                 eme:Currency ;
        rdfs:comment "Peruvian nuevo sol." ;
        rdfs:label "PEN"@en .


#-- PGK
eme:PGK rdf:type owl:NamedIndividual ,
                 eme:Currency ;
        rdfs:comment "Papua New Guinean kina." ;
        rdfs:label "PGK"@en .


#-- PHP
eme:PHP rdf:type owl:NamedIndividual ,
                 eme:Currency ;
        rdfs:comment "Philippine peso." ;
        rdfs:label "PHP"@en .


#-- PKR
eme:PKR rdf:type owl:NamedIndividual ,
                 eme:Currency ;
        rdfs:comment "Pakistani rupee." ;
        rdfs:label "PKR"@en .


#-- PLN
eme:PLN rdf:type owl:NamedIndividual ,
                 eme:Currency ;
        rdfs:comment "Polish zloty." ;
        rdfs:label "PLN"@en .


#-- PYG
eme:PYG rdf:type owl:NamedIndividual ,
                 eme:Currency ;
        rdfs:comment "Paraguayan guaran." ;
        rdfs:label "PYG"@en .


#-- Pa
eme:Pa rdf:type owl:NamedIndividual ,
                eme:UnitSymbol ;
       rdfs:comment "Pressure in pascals Nm. Note the absolute or relative measurement of pressure is implied with this entry. See below for more explicit forms." ;
       rdfs:label "Pa"@en .


#-- PaPers
eme:PaPers rdf:type owl:NamedIndividual ,
                    eme:UnitSymbol ;
           rdfs:comment "Pressure change rate in pascals per second." ;
           rdfs:label "PaPers"@en .


#-- Pas
eme:Pas rdf:type owl:NamedIndividual ,
                 eme:UnitSymbol ;
        rdfs:comment "Dynamic viscosity pascal seconds." ;
        rdfs:label "Pas"@en .


#-- Q
eme:Q rdf:type owl:NamedIndividual ,
               eme:UnitSymbol ;
      rdfs:comment "Quantity power Q." ;
      rdfs:label "Q"@en .


#-- QAR
eme:QAR rdf:type owl:NamedIndividual ,
                 eme:Currency ;
        rdfs:comment "Qatari rial." ;
        rdfs:label "QAR"@en .


#-- Qh
eme:Qh rdf:type owl:NamedIndividual ,
                eme:UnitSymbol ;
       rdfs:comment "Quantity energy Qh." ;
       rdfs:label "Qh"@en .


#-- RON
eme:RON rdf:type owl:NamedIndividual ,
                 eme:Currency ;
        rdfs:comment "Romanian new leu." ;
        rdfs:label "RON"@en .


#-- RSD
eme:RSD rdf:type owl:NamedIndividual ,
                 eme:Currency ;
        rdfs:comment "Serbian dinar." ;
        rdfs:label "RSD"@en .


#-- RUB
eme:RUB rdf:type owl:NamedIndividual ,
                 eme:Currency ;
        rdfs:comment "Russian rouble." ;
        rdfs:label "RUB"@en .


#-- RWF
eme:RWF rdf:type owl:NamedIndividual ,
                 eme:Currency ;
        rdfs:comment "Rwandan franc." ;
        rdfs:label "RWF"@en .


#-- S
eme:S rdf:type owl:NamedIndividual ,
               eme:UnitSymbol ;
      rdfs:comment "Conductance in siemens." ;
      rdfs:label "S"@en .


#-- SAR
eme:SAR rdf:type owl:NamedIndividual ,
                 eme:Currency ;
        rdfs:comment "Saudi riyal." ;
        rdfs:label "SAR"@en .


#-- SBD
eme:SBD rdf:type owl:NamedIndividual ,
                 eme:Currency ;
        rdfs:comment "Solomon Islands dollar." ;
        rdfs:label "SBD"@en .


#-- SCR
eme:SCR rdf:type owl:NamedIndividual ,
                 eme:Currency ;
        rdfs:comment "Seychelles rupee." ;
        rdfs:label "SCR"@en .


#-- SDG
eme:SDG rdf:type owl:NamedIndividual ,
                 eme:Currency ;
        rdfs:comment "Sudanese pound." ;
        rdfs:label "SDG"@en .


#-- SEK
eme:SEK rdf:type owl:NamedIndividual ,
                 eme:Currency ;
        rdfs:comment "Swedish kronakronor." ;
        rdfs:label "SEK"@en .


#-- SGD
eme:SGD rdf:type owl:NamedIndividual ,
                 eme:Currency ;
        rdfs:comment "Singapore dollar." ;
        rdfs:label "SGD"@en .


#-- SHP
eme:SHP rdf:type owl:NamedIndividual ,
                 eme:Currency ;
        rdfs:comment "Saint Helena pound." ;
        rdfs:label "SHP"@en .


#-- SLL
eme:SLL rdf:type owl:NamedIndividual ,
                 eme:Currency ;
        rdfs:comment "Sierra Leonean leone." ;
        rdfs:label "SLL"@en .


#-- SOS
eme:SOS rdf:type owl:NamedIndividual ,
                 eme:Currency ;
        rdfs:comment "Somali shilling." ;
        rdfs:label "SOS"@en .


#-- SPerm
eme:SPerm rdf:type owl:NamedIndividual ,
                   eme:UnitSymbol ;
          rdfs:comment "Conductance per length Fm." ;
          rdfs:label "SPerm"@en .


#-- SRD
eme:SRD rdf:type owl:NamedIndividual ,
                 eme:Currency ;
        rdfs:comment "Surinamese dollar." ;
        rdfs:label "SRD"@en .


#-- STD
eme:STD rdf:type owl:NamedIndividual ,
                 eme:Currency ;
        rdfs:comment "So Tom and Prncipe dobra." ;
        rdfs:label "STD"@en .


#-- SYP
eme:SYP rdf:type owl:NamedIndividual ,
                 eme:Currency ;
        rdfs:comment "Syrian pound." ;
        rdfs:label "SYP"@en .


#-- SZL
eme:SZL rdf:type owl:NamedIndividual ,
                 eme:Currency ;
        rdfs:comment "Lilangeni." ;
        rdfs:label "SZL"@en .


#-- Sv
eme:Sv rdf:type owl:NamedIndividual ,
                eme:UnitSymbol ;
       rdfs:comment "Dose equivalent in sieverts Jkg." ;
       rdfs:label "Sv"@en .


#-- T
eme:T rdf:type owl:NamedIndividual ,
               eme:UnitMultiplier ,
               eme:UnitSymbol ;
      rdfs:comment "Magnetic flux density in teslas Wbm2." ,
                   "Tera 1012." ;
      rdfs:label "T"@en .


#-- THB
eme:THB rdf:type owl:NamedIndividual ,
                 eme:Currency ;
        rdfs:comment "Thai baht." ;
        rdfs:label "THB"@en .


#-- TJS
eme:TJS rdf:type owl:NamedIndividual ,
                 eme:Currency ;
        rdfs:comment "Tajikistani somoni." ;
        rdfs:label "TJS"@en .


#-- TMT
eme:TMT rdf:type owl:NamedIndividual ,
                 eme:Currency ;
        rdfs:comment "Turkmenistani manat." ;
        rdfs:label "TMT"@en .


#-- TND
eme:TND rdf:type owl:NamedIndividual ,
                 eme:Currency ;
        rdfs:comment "Tunisian dinar." ;
        rdfs:label "TND"@en .


#-- TOP
eme:TOP rdf:type owl:NamedIndividual ,
                 eme:Currency ;
        rdfs:comment "Tongan paanga." ;
        rdfs:label "TOP"@en .


#-- TRY
eme:TRY rdf:type owl:NamedIndividual ,
                 eme:Currency ;
        rdfs:comment "Turkish lira." ;
        rdfs:label "TRY"@en .


#-- TTD
eme:TTD rdf:type owl:NamedIndividual ,
                 eme:Currency ;
        rdfs:comment "Trinidad and Tobago dollar." ;
        rdfs:label "TTD"@en .


#-- TWD
eme:TWD rdf:type owl:NamedIndividual ,
                 eme:Currency ;
        rdfs:comment "New Taiwan dollar." ;
        rdfs:label "TWD"@en .


#-- TZS
eme:TZS rdf:type owl:NamedIndividual ,
                 eme:Currency ;
        rdfs:comment "Tanzanian shilling." ;
        rdfs:label "TZS"@en .


#-- UAH
eme:UAH rdf:type owl:NamedIndividual ,
                 eme:Currency ;
        rdfs:comment "Ukrainian hryvnia." ;
        rdfs:label "UAH"@en .


#-- UGX
eme:UGX rdf:type owl:NamedIndividual ,
                 eme:Currency ;
        rdfs:comment "Ugandan shilling." ;
        rdfs:label "UGX"@en .


#-- USD
eme:USD rdf:type owl:NamedIndividual ,
                 eme:Currency ;
        rdfs:comment "United States dollar." ;
        rdfs:label "USD"@en .


#-- UYU
eme:UYU rdf:type owl:NamedIndividual ,
                 eme:Currency ;
        rdfs:comment "Uruguayan peso." ;
        rdfs:label "UYU"@en .


#-- UZS
eme:UZS rdf:type owl:NamedIndividual ,
                 eme:Currency ;
        rdfs:comment "Uzbekistan som." ;
        rdfs:label "UZS"@en .


#-- V
eme:V rdf:type owl:NamedIndividual ,
               eme:UnitSymbol ;
      rdfs:comment "Electric potential in volts WA." ;
      rdfs:label "V"@en .


#-- V2
eme:V2 rdf:type owl:NamedIndividual ,
                eme:UnitSymbol ;
       rdfs:comment "Volt squared WA." ;
       rdfs:label "V2"@en .


#-- V2h
eme:V2h rdf:type owl:NamedIndividual ,
                 eme:UnitSymbol ;
        rdfs:comment "Voltsquared hour voltsquaredhours." ;
        rdfs:label "V2h"@en .


#-- VA
eme:VA rdf:type owl:NamedIndividual ,
                eme:UnitSymbol ;
       rdfs:comment "Apparent power in volt amperes. See also real power and reactive power." ;
       rdfs:label "VA"@en .


#-- VAh
eme:VAh rdf:type owl:NamedIndividual ,
                 eme:UnitSymbol ;
        rdfs:comment "Apparent energy in volt ampere hours." ;
        rdfs:label "VAh"@en .


#-- VAr
eme:VAr rdf:type owl:NamedIndividual ,
                 eme:UnitSymbol ;
        rdfs:comment "Reactive power in volt amperes reactive. The reactive or imaginary component of electrical power VIsinphi. See also real power and apparent power.Note Different meter designs use different methods to arrive at their results. Some meters may compute reactive power as an arithmetic value while others compute the value vectorially. The data consumer should determine the method in use and the suitability of the measurement for the intended purpose." ;
        rdfs:label "VAr"@en .


#-- VArh
eme:VArh rdf:type owl:NamedIndividual ,
                  eme:UnitSymbol ;
         rdfs:comment "Reactive energy in volt ampere reactive hours." ;
         rdfs:label "VArh"@en .


#-- VEF
eme:VEF rdf:type owl:NamedIndividual ,
                 eme:Currency ;
        rdfs:comment "Venezuelan bolvar fuerte." ;
        rdfs:label "VEF"@en .


#-- VND
eme:VND rdf:type owl:NamedIndividual ,
                 eme:Currency ;
        rdfs:comment "Vietnamese Dong." ;
        rdfs:label "VND"@en .


#-- VPerHz
eme:VPerHz rdf:type owl:NamedIndividual ,
                    eme:UnitSymbol ;
           rdfs:comment "Magnetic flux in volt per hertz." ;
           rdfs:label "VPerHz"@en .


#-- VPerV
eme:VPerV rdf:type owl:NamedIndividual ,
                   eme:UnitSymbol ;
          rdfs:comment "Voltage ratio of voltages.  Note Users may need to supply a prefix such as m to show rates such as mVV." ;
          rdfs:label "VPerV"@en .


#-- VPerVA
eme:VPerVA rdf:type owl:NamedIndividual ,
                    eme:UnitSymbol ;
           rdfs:comment "Power factor PF the ratio of the active power to the apparent power.  Note The sign convention used for power factor will differ between IEC meters and EEI ANSI meters. It is assumed that the data consumers understand the type of meter being used and agree on the sign convention in use at any given utility." ;
           rdfs:label "VPerVA"@en .


#-- VPerVAr
eme:VPerVAr rdf:type owl:NamedIndividual ,
                     eme:UnitSymbol ;
            rdfs:comment "Power factor PF the ratio of the active power to the apparent power. Note The sign convention used for power factor will differ between IEC meters and EEI ANSI meters. It is assumed that the data consumers understand the type of meter being used and agree on the sign convention in use at any given utility." ;
            rdfs:label "VPerVAr"@en .


#-- VPerm
eme:VPerm rdf:type owl:NamedIndividual ,
                   eme:UnitSymbol ;
          rdfs:comment "Electric field strength volts per metre." ;
          rdfs:label "VPerm"@en .


#-- VUV
eme:VUV rdf:type owl:NamedIndividual ,
                 eme:Currency ;
        rdfs:comment "Vanuatu vatu." ;
        rdfs:label "VUV"@en .


#-- Vh
eme:Vh rdf:type owl:NamedIndividual ,
                eme:UnitSymbol ;
       rdfs:comment "Volthour Volt hours." ;
       rdfs:label "Vh"@en .


#-- Vs
eme:Vs rdf:type owl:NamedIndividual ,
                eme:UnitSymbol ;
       rdfs:comment "Volt seconds WsA." ;
       rdfs:label "Vs"@en .


#-- W
eme:W rdf:type owl:NamedIndividual ,
               eme:UnitSymbol ;
      rdfs:comment "Real power in watts Js. Electrical power may have real and reactive components. The real portion of electrical power I178R or VIcosphi is expressed in Watts. See also apparent power and reactive power." ;
      rdfs:label "W"@en .


#-- WPerA
eme:WPerA rdf:type owl:NamedIndividual ,
                   eme:UnitSymbol ;
          rdfs:comment "Active power per current flow watts per Ampere." ;
          rdfs:label "WPerA"@en .


#-- WPerW
eme:WPerW rdf:type owl:NamedIndividual ,
                   eme:UnitSymbol ;
          rdfs:comment "Signal Strength ratio of power.   Note Users may need to supply a prefix such as m to show rates such as mWW." ;
          rdfs:label "WPerW"@en .


#-- WPerm2
eme:WPerm2 rdf:type owl:NamedIndividual ,
                    eme:UnitSymbol ;
           rdfs:comment "Heat flux density irradiance watts per square metre." ;
           rdfs:label "WPerm2"@en .


#-- WPerm2sr
eme:WPerm2sr rdf:type owl:NamedIndividual ,
                      eme:UnitSymbol ;
             rdfs:comment "Radiance watts per square metre steradian." ;
             rdfs:label "WPerm2sr"@en .


#-- WPermK
eme:WPermK rdf:type owl:NamedIndividual ,
                    eme:UnitSymbol ;
           rdfs:comment "Thermal conductivity in wattmetres kelvin." ;
           rdfs:label "WPermK"@en .


#-- WPers
eme:WPers rdf:type owl:NamedIndividual ,
                   eme:UnitSymbol ;
          rdfs:comment "Ramp rate in watts per second." ;
          rdfs:label "WPers"@en .


#-- WPersr
eme:WPersr rdf:type owl:NamedIndividual ,
                    eme:UnitSymbol ;
           rdfs:comment "Radiant intensity watts per steradian." ;
           rdfs:label "WPersr"@en .


#-- WST
eme:WST rdf:type owl:NamedIndividual ,
                 eme:Currency ;
        rdfs:comment "Samoan tala." ;
        rdfs:label "WST"@en .


#-- Wb
eme:Wb rdf:type owl:NamedIndividual ,
                eme:UnitSymbol ;
       rdfs:comment "Magnetic flux in webers Vs." ;
       rdfs:label "Wb"@en .


#-- Wh
eme:Wh rdf:type owl:NamedIndividual ,
                eme:UnitSymbol ;
       rdfs:comment "Real energy in watt hours." ;
       rdfs:label "Wh"@en .


#-- X
eme:X rdf:type owl:NamedIndividual ,
               eme:PhaseCode ;
      rdfs:comment "Unknown non-neutral phase."@en .


#-- XAF
eme:XAF rdf:type owl:NamedIndividual ,
                 eme:Currency ;
        rdfs:comment "CFA franc BEAC." ;
        rdfs:label "XAF"@en .


#-- XCD
eme:XCD rdf:type owl:NamedIndividual ,
                 eme:Currency ;
        rdfs:comment "East Caribbean dollar." ;
        rdfs:label "XCD"@en .


#-- XN
eme:XN rdf:type owl:NamedIndividual ,
                eme:PhaseCode ;
       rdfs:comment "Unknown non-neutral phase plus neutral."@en .


#-- XOF
eme:XOF rdf:type owl:NamedIndividual ,
                 eme:Currency ;
        rdfs:comment "CFA Franc BCEAO." ;
        rdfs:label "XOF"@en .


#-- XPF
eme:XPF rdf:type owl:NamedIndividual ,
                 eme:Currency ;
        rdfs:comment "CFP franc." ;
        rdfs:label "XPF"@en .


#-- XY
eme:XY rdf:type owl:NamedIndividual ,
                eme:PhaseCode ;
       rdfs:comment "Two unknown non-neutral phases."@en .


#-- XYN
eme:XYN rdf:type owl:NamedIndividual ,
                 eme:PhaseCode ;
        rdfs:comment "Two unknown non-neutral phases plus neutral."@en .


#-- Y
eme:Y rdf:type owl:NamedIndividual ,
               eme:UnitMultiplier ;
      rdfs:comment "Yotta 1024." ;
      rdfs:label "Y"@en .


#-- YER
eme:YER rdf:type owl:NamedIndividual ,
                 eme:Currency ;
        rdfs:comment "Yemeni rial." ;
        rdfs:label "YER"@en .


#-- Z
eme:Z rdf:type owl:NamedIndividual ,
               eme:UnitMultiplier ;
      rdfs:comment "Zetta 1021." ;
      rdfs:label "Z"@en .


#-- ZAR
eme:ZAR rdf:type owl:NamedIndividual ,
                 eme:Currency ;
        rdfs:comment "South African rand." ;
        rdfs:label "ZAR"@en .


#-- ZMK
eme:ZMK rdf:type owl:NamedIndividual ,
                 eme:Currency ;
        rdfs:comment "Zambian kwacha." ;
        rdfs:label "ZMK"@en .


#-- ZWL
eme:ZWL rdf:type owl:NamedIndividual ,
                 eme:Currency ;
        rdfs:comment "Zimbabwe dollar." ;
        rdfs:label "ZWL"@en .


#-- a
eme:a rdf:type owl:NamedIndividual ,
               eme:UnitMultiplier ;
      rdfs:comment "Atto 1018." ;
      rdfs:label "a"@en .


#-- air
eme:air rdf:type owl:NamedIndividual ,
                 eme:CommodityKind .


#-- alarm
eme:alarm rdf:type owl:NamedIndividual ,
                   eme:MeasurementKind ;
          rdfs:label "alarm"@en .


#-- anglemin
eme:anglemin rdf:type owl:NamedIndividual ,
                      eme:UnitSymbol ;
             rdfs:comment "Plane angle minutes." ;
             rdfs:label "anglemin"@en .


#-- anglesec
eme:anglesec rdf:type owl:NamedIndividual ,
                      eme:UnitSymbol ;
             rdfs:comment "Plane angle seconds." ;
             rdfs:label "anglesec"@en .


#-- apTitle
eme:apTitle rdf:type owl:NamedIndividual ,
                     eme:MeasurementKind ;
            rdfs:label "apTitle"@en .


#-- apparentPowerFactor
eme:apparentPowerFactor rdf:type owl:NamedIndividual ,
                                 eme:MeasurementKind ;
                        rdfs:label "apparentPowerFactor"@en .


#-- applicationContext
eme:applicationContext rdf:type owl:NamedIndividual ,
                                eme:MeasurementKind ;
                       rdfs:label "applicationContext"@en .


#-- assetNumber
eme:assetNumber rdf:type owl:NamedIndividual ,
                         eme:MeasurementKind ;
                rdfs:label "assetNumber"@en .


#-- audibleVolume
eme:audibleVolume rdf:type owl:NamedIndividual ,
                           eme:MeasurementKind ;
                  rdfs:comment "Sound" ;
                  rdfs:label "audibleVolume"@en .


#-- average
eme:average rdf:type owl:NamedIndividual ,
                     eme:AggregateKind ;
            rdfs:comment "The value represents average."@en .


#-- bandwidth
eme:bandwidth rdf:type owl:NamedIndividual ,
                       eme:MeasurementKind ;
              rdfs:label "bandwidth"@en .


#-- bar
eme:bar rdf:type owl:NamedIndividual ,
                 eme:UnitSymbol ;
        rdfs:comment "Pressure in bars 1 bar  100 kPa." ;
        rdfs:label "bar"@en .


#-- batteryCarryover
eme:batteryCarryover rdf:type owl:NamedIndividual ,
                              eme:MeasurementKind ;
                     rdfs:label "batteryCarryover"@en .


#-- batteryVoltage
eme:batteryVoltage rdf:type owl:NamedIndividual ,
                            eme:MeasurementKind ;
                   rdfs:label "batteryVoltage"@en .


#-- billCarryover
eme:billCarryover rdf:type owl:NamedIndividual ,
                           eme:MeasurementKind ;
                  rdfs:comment "Customers bill for the Currency" ;
                  rdfs:label "billCarryover"@en .


#-- billLastPeriod
eme:billLastPeriod rdf:type owl:NamedIndividual ,
                            eme:MeasurementKind ;
                   rdfs:comment "Customers bill for the previous billing period Currency" ;
                   rdfs:label "billLastPeriod"@en .


#-- billToDate
eme:billToDate rdf:type owl:NamedIndividual ,
                        eme:MeasurementKind ;
               rdfs:comment "Customers bill as known thus far within the present billing period Currency" ;
               rdfs:label "billToDate"@en .


#-- billingPeriod
eme:billingPeriod rdf:type owl:NamedIndividual ,
                           eme:MacroPeriodKind ;
                  rdfs:comment "Captured during the billing period starting at midnight of the first day of the billing period (as defined by the billing cycle day). If during the current billing period, it specifies a period from the start of the current billing period until \"now\"."@en .


#-- boundedQuantity
eme:boundedQuantity rdf:type owl:NamedIndividual ,
                             eme:AccumulationKind ;
                    rdfs:comment "A time-independent cumulative quantity much like a 'bulkQuantity' or a 'latchingQuantity', except that the accumulation stops at the maximum or minimum values. When the maximum is reached, any additional positive accumulation is discarded, but negative accumulation may be accepted (thus lowering the counter.) Likewise, when the negative bound is reached, any additional negative accumulation is discarded, but positive accumulation is accepted (thus increasing the counter.)"@en .


#-- broadcastAddress
eme:broadcastAddress rdf:type owl:NamedIndividual ,
                              eme:MeasurementKind ;
                     rdfs:label "broadcastAddress"@en .


#-- bulkQuantity
eme:bulkQuantity rdf:type owl:NamedIndividual ,
                          eme:AccumulationKind ;
                 rdfs:comment """A value from a register which represents the bulk quantity of a commodity. This quantity is computed as the integral of the commodity usage rate. This value is typically used as the basis for the dial reading at the meter, and as a result, will roll over upon reaching a maximum dial value. 
Note 1: With the metering system, the roll-over behaviour typically implies a roll-under behavior so that the value presented is always a positive value (e.g. unsigned integer or positive decimal.) However, when communicating data between enterprise applications a negative value might occur in a case such as net metering.
Note 2: A 'bulkQuantity' refers primarily to the dial reading and not the consumption over a specific period of time."""@en .


#-- c
eme:c rdf:type owl:NamedIndividual ,
               eme:UnitMultiplier ;
      rdfs:comment "Centi 102." ;
      rdfs:label "c"@en .


#-- carbon
eme:carbon rdf:type owl:NamedIndividual ,
                    eme:CommodityKind .


#-- cd
eme:cd rdf:type owl:NamedIndividual ,
                eme:UnitSymbol ;
       rdfs:comment "Luminous intensity in candelas." ;
       rdfs:label "cd"@en .


#-- ch4
eme:ch4 rdf:type owl:NamedIndividual ,
                 eme:CommodityKind ;
        rdfs:comment "Methane CH4"@en .


#-- charPers
eme:charPers rdf:type owl:NamedIndividual ,
                      eme:UnitSymbol ;
             rdfs:comment "Data rate baud in characters per second." ;
             rdfs:label "charPers"@en .


#-- character
eme:character rdf:type owl:NamedIndividual ,
                       eme:UnitSymbol ;
              rdfs:comment "Number of characters." ;
              rdfs:label "character"@en .


#-- co2
eme:co2 rdf:type owl:NamedIndividual ,
                 eme:CommodityKind ;
        rdfs:comment "Carbon Dioxide CO2"@en .


#-- commercialIndustrial
eme:commercialIndustrial rdf:type owl:NamedIndividual ,
                                  eme:CustomerKind ;
                         rdfs:comment "Commercial industrial customer."@en .


#-- communication
eme:communication rdf:type owl:NamedIndividual ,
                           eme:CommodityKind ;
                  rdfs:comment "A measurement of the communication infrastructure itself."@en .


#-- connectionFee
eme:connectionFee rdf:type owl:NamedIndividual ,
                           eme:MeasurementKind ;
                  rdfs:comment "Monthly fee for connection to commodity." ;
                  rdfs:label "connectionFee"@en .


#-- continuousCumulative
eme:continuousCumulative rdf:type owl:NamedIndividual ,
                                  eme:AccumulationKind ;
                         rdfs:comment """The sum of the previous billing period values and the present period value.
Note: 'continuousCumulative' is commonly used in conjunction with 'demand', and it  would represent the cumulative sum of the previous billing period maximum demand values (as occurring with each demand reset) summed with the present period maximum demand value (which has yet to be reset.)"""@en .


#-- coolingFluid
eme:coolingFluid rdf:type owl:NamedIndividual ,
                          eme:CommodityKind ;
                 rdfs:comment "The cool fluid returns warmer than when it was sent. The heat conveyed may be metered."@en .


#-- cosPhi
eme:cosPhi rdf:type owl:NamedIndividual ,
                    eme:UnitSymbol ;
           rdfs:comment "Power factor dimensionless.Note 1 This definition of power factor only holds for balanced systems. See the alternative definition under code 153.Note 2 Beware of differing sign conventions in use between the IEC and EEI. It is assumed that the data consumer understands the type of meter in use and the sign convention in use by the utility." ;
           rdfs:label "cosPhi"@en .


#-- count
eme:count rdf:type owl:NamedIndividual ,
                   eme:UnitSymbol ;
          rdfs:comment "Amount of substance Counter value." ;
          rdfs:label "count"@en .


#-- cumulative
eme:cumulative rdf:type owl:NamedIndividual ,
                        eme:AccumulationKind ;
               rdfs:comment """The sum of the previous billing period values.
Note: 'cumulative' is commonly used in conjunction with “demand.” Each demand reset causes the maximum demand value for the present billing period (since the last demand reset) to accumulate as an accumulative total of all maximum demands. So instead of 'zeroing' the demand register, a demand reset has the effect of adding the present maximum demand to this accumulating total."""@en .


#-- currency
eme:currency rdf:type owl:NamedIndividual ,
                      eme:MeasurementKind ;
             rdfs:comment "funds" ;
             rdfs:label "currency"@en .


#-- current
eme:current rdf:type owl:NamedIndividual ,
                     eme:MeasurementKind ;
            rdfs:label "current"@en .


#-- currentAngle
eme:currentAngle rdf:type owl:NamedIndividual ,
                          eme:MeasurementKind ;
                 rdfs:label "currentAngle"@en .


#-- currentImbalance
eme:currentImbalance rdf:type owl:NamedIndividual ,
                              eme:MeasurementKind ;
                     rdfs:label "currentImbalance"@en .


#-- d
eme:d rdf:type owl:NamedIndividual ,
               eme:UnitMultiplier ,
               eme:UnitSymbol ;
      rdfs:comment "Deci 101." ,
                   "Time in days day  24 h  86400 s." ;
      rdfs:label "d"@en .


#-- dB
eme:dB rdf:type owl:NamedIndividual ,
                eme:UnitSymbol ;
       rdfs:comment "Sound pressure level in decibels. Note  multiplier d is included in this unit symbol for compatibility with IEC 6185073." ;
       rdfs:label "dB"@en .


#-- dBm
eme:dBm rdf:type owl:NamedIndividual ,
                 eme:UnitSymbol ;
        rdfs:comment "Power level logarithmic ratio of signal strength  BelmW normalized to 1mW. Note  multiplier d is included in this unit symbol for compatibility with IEC 6185073." ;
        rdfs:label "dBm"@en .


#-- da
eme:da rdf:type owl:NamedIndividual ,
                eme:UnitMultiplier ;
       rdfs:comment "Deca 101." ;
       rdfs:label "da"@en .


#-- daily
eme:daily rdf:type owl:NamedIndividual ,
                   eme:MacroPeriodKind ;
          rdfs:comment "Daily period starting at midnight. If for the current day, this specifies the time from midnight to \"now\"."@en .


#-- dataOverflowAlarm
eme:dataOverflowAlarm rdf:type owl:NamedIndividual ,
                               eme:MeasurementKind ;
                      rdfs:label "dataOverflowAlarm"@en .


#-- date
eme:date rdf:type owl:NamedIndividual ,
                  eme:MeasurementKind ;
         rdfs:label "date"@en .


#-- deg
eme:deg rdf:type owl:NamedIndividual ,
                 eme:UnitSymbol ;
        rdfs:comment "Plane angle in degrees." ;
        rdfs:label "deg"@en .


#-- degC
eme:degC rdf:type owl:NamedIndividual ,
                  eme:UnitSymbol ;
         rdfs:comment "Relative temperature in degrees Celsius.In the SI unit system the symbol is C. Electric charge is measured in coulomb that has the unit symbol C. To distinguish degree Celsius from coulomb the symbol used in the UML is degC. The reason for not using C is that the special character  is difficult to manage in software." ;
         rdfs:label "degC"@en .


#-- deltaData
eme:deltaData rdf:type owl:NamedIndividual ,
                       eme:AccumulationKind ;
              rdfs:comment """The difference between the value at the end of the prescribed interval and the beginning of the interval. This is used for incremental interval data. 
Note: One common application would be for load profile data, another use might be to report the number of events within an interval (such as the number of equipment energisations within the specified period of time.)"""@en .


#-- demand
eme:demand rdf:type owl:NamedIndividual ,
                    eme:MeasurementKind ;
           rdfs:label "demand"@en .


#-- demandLimit
eme:demandLimit rdf:type owl:NamedIndividual ,
                         eme:MeasurementKind ;
                rdfs:label "demandLimit"@en .


#-- demandReset
eme:demandReset rdf:type owl:NamedIndividual ,
                         eme:MeasurementKind ;
                rdfs:comment "Usually expressed as a count as part of a billing cycle" ;
                rdfs:label "demandReset"@en .


#-- deviceAddressType1
eme:deviceAddressType1 rdf:type owl:NamedIndividual ,
                                eme:MeasurementKind ;
                       rdfs:label "deviceAddressType1"@en .


#-- deviceAddressType2
eme:deviceAddressType2 rdf:type owl:NamedIndividual ,
                                eme:MeasurementKind ;
                       rdfs:label "deviceAddressType2"@en .


#-- deviceAddressType3
eme:deviceAddressType3 rdf:type owl:NamedIndividual ,
                                eme:MeasurementKind ;
                       rdfs:label "deviceAddressType3"@en .


#-- deviceAddressType4
eme:deviceAddressType4 rdf:type owl:NamedIndividual ,
                                eme:MeasurementKind ;
                       rdfs:label "deviceAddressType4"@en .


#-- deviceClass
eme:deviceClass rdf:type owl:NamedIndividual ,
                         eme:MeasurementKind ;
                rdfs:label "deviceClass"@en .


#-- diagnostic
eme:diagnostic rdf:type owl:NamedIndividual ,
                        eme:MeasurementKind ;
               rdfs:label "diagnostic"@en .


#-- distance
eme:distance rdf:type owl:NamedIndividual ,
                      eme:MeasurementKind ;
             rdfs:label "distance"@en .


#-- distortionPowerFactor
eme:distortionPowerFactor rdf:type owl:NamedIndividual ,
                                   eme:MeasurementKind ;
                          rdfs:label "distortionPowerFactor"@en .


#-- distortionVoltAmp
eme:distortionVoltAmp rdf:type owl:NamedIndividual ,
                               eme:MeasurementKind ;
                      rdfs:label "distortionVoltAmp"@en .


#-- electricityPrimaryMetered
eme:electricityPrimaryMetered rdf:type owl:NamedIndividual ,
                                       eme:CommodityKind ;
                              rdfs:comment "It is possible for a meter to be outfitted with an external VT and/or CT. The meter might not be aware of these devices, and the display not compensate for their presence. Ultimately, when these scalars are applied, the value that represents the service value is called the “primary metered” value. The “index” in sub-category 3 mirrors those of sub-category 0."@en .


#-- electricitySecondaryMetered
eme:electricitySecondaryMetered rdf:type owl:NamedIndividual ,
                                         eme:CommodityKind ;
                                rdfs:comment "All types of metered quantities. This type of reading comes from the meter and represents a “secondary” metered value."@en .


#-- electronicSerialNumber
eme:electronicSerialNumber rdf:type owl:NamedIndividual ,
                                    eme:MeasurementKind ;
                           rdfs:label "electronicSerialNumber"@en .


#-- emergencyLimit
eme:emergencyLimit rdf:type owl:NamedIndividual ,
                            eme:MeasurementKind ;
                   rdfs:label "emergencyLimit"@en .


#-- encoderTamper
eme:encoderTamper rdf:type owl:NamedIndividual ,
                           eme:MeasurementKind ;
                  rdfs:label "encoderTamper"@en .


#-- endDeviceID
eme:endDeviceID rdf:type owl:NamedIndividual ,
                         eme:MeasurementKind ;
                rdfs:label "endDeviceID"@en .


#-- energization
eme:energization rdf:type owl:NamedIndividual ,
                          eme:MeasurementKind ;
                 rdfs:label "energization"@en .


#-- energizationLoadSide
eme:energizationLoadSide rdf:type owl:NamedIndividual ,
                                  eme:MeasurementKind ;
                         rdfs:label "energizationLoadSide"@en .


#-- energy
eme:energy rdf:type owl:NamedIndividual ,
                    eme:MeasurementKind ;
           rdfs:label "energy"@en .


#-- energyServiceScheduler
eme:energyServiceScheduler rdf:type owl:NamedIndividual ,
                                    eme:CustomerKind ;
                           rdfs:comment "Customer as energy service scheduler."@en .


#-- energyServiceSupplier
eme:energyServiceSupplier rdf:type owl:NamedIndividual ,
                                   eme:CustomerKind ;
                          rdfs:comment "Customer as energy service supplier."@en .


#-- excess
eme:excess rdf:type owl:NamedIndividual ,
                    eme:AggregateKind ;
           rdfs:comment "The value represents an amount over which a threshold was exceeded."@en .


#-- f
eme:f rdf:type owl:NamedIndividual ,
               eme:UnitMultiplier ;
      rdfs:comment "Femto 1015." ;
      rdfs:label "f"@en .


#-- fan
eme:fan rdf:type owl:NamedIndividual ,
                 eme:MeasurementKind ;
        rdfs:label "fan"@en .


#-- fifteenMinute
eme:fifteenMinute rdf:type owl:NamedIndividual ,
                           eme:MeasuringPeriodKind ;
                  rdfs:comment "15-minute"@en .


#-- fifthMaximum
eme:fifthMaximum rdf:type owl:NamedIndividual ,
                          eme:AggregateKind ;
                 rdfs:comment "The fifth highest value observed."@en .


#-- fiveMinute
eme:fiveMinute rdf:type owl:NamedIndividual ,
                        eme:MeasuringPeriodKind ;
               rdfs:comment "5-minute" .


#-- fixedBlock10Min
eme:fixedBlock10Min rdf:type owl:NamedIndividual ,
                             eme:MeasuringPeriodKind ;
                    rdfs:comment "10-minute Fixed Block"@en .


#-- fixedBlock15Min
eme:fixedBlock15Min rdf:type owl:NamedIndividual ,
                             eme:MeasuringPeriodKind ;
                    rdfs:comment "15-minute Fixed Block"@en .


#-- fixedBlock1Min
eme:fixedBlock1Min rdf:type owl:NamedIndividual ,
                            eme:MeasuringPeriodKind ;
                   rdfs:comment "1-minute Fixed Block"@en .


#-- fixedBlock20Min
eme:fixedBlock20Min rdf:type owl:NamedIndividual ,
                             eme:MeasuringPeriodKind ;
                    rdfs:comment "20-minute Fixed Block"@en .


#-- fixedBlock30Min
eme:fixedBlock30Min rdf:type owl:NamedIndividual ,
                             eme:MeasuringPeriodKind ;
                    rdfs:comment "30-minute Fixed Block"@en .


#-- fixedBlock5Min
eme:fixedBlock5Min rdf:type owl:NamedIndividual ,
                            eme:MeasuringPeriodKind ;
                   rdfs:comment "5-minute Fixed Block"@en .


#-- fixedBlock60Min
eme:fixedBlock60Min rdf:type owl:NamedIndividual ,
                             eme:MeasuringPeriodKind ;
                    rdfs:comment "60-minute Fixed Block"@en .


#-- forward
eme:forward rdf:type owl:NamedIndividual ,
                     eme:FlowDirectionKind ;
            rdfs:comment """\"Delivered,\" or \"Imported\" as defined 61968-2.
Forward Active Energy is a positive kWh value as one would naturally expect to find as energy is supplied by the utility and consumed at the service.
Forward Reactive Energy is a positive VArh value as one would naturally expect to find in the presence of inductive loading.
In polyphase metering, the forward energy register is incremented when the sum of the phase energies is greater than zero:
<img src=\"HTS_1.PNG\" width=\"209\" height=\"16\" border=\"0\" alt=\"graphic\"/>"""@en .


#-- fourthMaximum
eme:fourthMaximum rdf:type owl:NamedIndividual ,
                           eme:AggregateKind ;
                  rdfs:comment "The fourth highest value observed."@en .


#-- frequency
eme:frequency rdf:type owl:NamedIndividual ,
                       eme:MeasurementKind ;
              rdfs:label "frequency"@en .


#-- frequencyExcursion
eme:frequencyExcursion rdf:type owl:NamedIndividual ,
                                eme:MeasurementKind ;
                       rdfs:comment "Usually expressed as a count" ;
                       rdfs:label "frequencyExcursion"@en .


#-- ft3
eme:ft3 rdf:type owl:NamedIndividual ,
                 eme:UnitSymbol ;
        rdfs:comment "Volume cubic feet." ;
        rdfs:label "ft3"@en .


#-- fund
eme:fund rdf:type owl:NamedIndividual ,
                  eme:MeasurementKind ;
         rdfs:comment "Dup with currency" ;
         rdfs:label "fund"@en .


#-- gPerg
eme:gPerg rdf:type owl:NamedIndividual ,
                   eme:UnitSymbol ;
          rdfs:comment "Concentration The ratio of the mass of a solute divided by the mass of  the solution. Note Users may need use a prefix such a  to express a quantity such as gg." ;
          rdfs:label "gPerg"@en .


#-- gal
eme:gal rdf:type owl:NamedIndividual ,
                 eme:UnitSymbol ;
        rdfs:comment "Volume in gallons US gallon 1 gal  231 in3  128 fl ounce." ;
        rdfs:label "gal"@en .


#-- groupAddressType1
eme:groupAddressType1 rdf:type owl:NamedIndividual ,
                               eme:MeasurementKind ;
                      rdfs:label "groupAddressType1"@en .


#-- groupAddressType2
eme:groupAddressType2 rdf:type owl:NamedIndividual ,
                               eme:MeasurementKind ;
                      rdfs:label "groupAddressType2"@en .


#-- groupAddressType3
eme:groupAddressType3 rdf:type owl:NamedIndividual ,
                               eme:MeasurementKind ;
                      rdfs:label "groupAddressType3"@en .


#-- groupAddressType4
eme:groupAddressType4 rdf:type owl:NamedIndividual ,
                               eme:MeasurementKind ;
                      rdfs:label "groupAddressType4"@en .


#-- h
eme:h rdf:type owl:NamedIndividual ,
               eme:UnitMultiplier ,
               eme:UnitSymbol ;
      rdfs:comment "Hecto 102." ,
                   "Time in hours hour  60 min  3600 s." ;
      rdfs:label "h"@en .


#-- ha
eme:ha rdf:type owl:NamedIndividual ,
                eme:UnitSymbol ;
       rdfs:comment "Area hectares." ;
       rdfs:label "ha"@en .


#-- hch
eme:hch rdf:type owl:NamedIndividual ,
                 eme:CommodityKind ;
        rdfs:comment "Hexachlorocyclohexane HCH"@en .


#-- heatingFluid
eme:heatingFluid rdf:type owl:NamedIndividual ,
                          eme:CommodityKind ;
                 rdfs:comment "This fluid is likely in liquid form. It is not necessarily water or water based. The warm fluid returns cooler than when it was sent. The heat conveyed may be metered."@en .


#-- highThreshold
eme:highThreshold rdf:type owl:NamedIndividual ,
                           eme:AggregateKind ;
                  rdfs:comment "The value represents a programmed high threshold."@en .


#-- ieee1366ASAI
eme:ieee1366ASAI rdf:type owl:NamedIndividual ,
                          eme:MeasurementKind ;
                 rdfs:label "ieee1366ASAI"@en .


#-- ieee1366ASIDI
eme:ieee1366ASIDI rdf:type owl:NamedIndividual ,
                           eme:MeasurementKind ;
                  rdfs:label "ieee1366ASIDI"@en .


#-- ieee1366ASIFI
eme:ieee1366ASIFI rdf:type owl:NamedIndividual ,
                           eme:MeasurementKind ;
                  rdfs:label "ieee1366ASIFI"@en .


#-- ieee1366CAIDI
eme:ieee1366CAIDI rdf:type owl:NamedIndividual ,
                           eme:MeasurementKind ;
                  rdfs:label "ieee1366CAIDI"@en .


#-- ieee1366CAIFI
eme:ieee1366CAIFI rdf:type owl:NamedIndividual ,
                           eme:MeasurementKind ;
                  rdfs:label "ieee1366CAIFI"@en .


#-- ieee1366CEMIn
eme:ieee1366CEMIn rdf:type owl:NamedIndividual ,
                           eme:MeasurementKind ;
                  rdfs:label "ieee1366CEMIn"@en .


#-- ieee1366CEMSMIn
eme:ieee1366CEMSMIn rdf:type owl:NamedIndividual ,
                             eme:MeasurementKind ;
                    rdfs:label "ieee1366CEMSMIn"@en .


#-- ieee1366CTAIDI
eme:ieee1366CTAIDI rdf:type owl:NamedIndividual ,
                            eme:MeasurementKind ;
                   rdfs:label "ieee1366CTAIDI"@en .


#-- ieee1366MAIFI
eme:ieee1366MAIFI rdf:type owl:NamedIndividual ,
                           eme:MeasurementKind ;
                  rdfs:label "ieee1366MAIFI"@en .


#-- ieee1366MAIFIe
eme:ieee1366MAIFIe rdf:type owl:NamedIndividual ,
                            eme:MeasurementKind ;
                   rdfs:label "ieee1366MAIFIe"@en .


#-- ieee1366MomentaryInterruption
eme:ieee1366MomentaryInterruption rdf:type owl:NamedIndividual ,
                                           eme:MeasurementKind ;
                                  rdfs:label "ieee1366MomentaryInterruption"@en .


#-- ieee1366MomentaryInterruptionEvent
eme:ieee1366MomentaryInterruptionEvent rdf:type owl:NamedIndividual ,
                                                eme:MeasurementKind ;
                                       rdfs:label "ieee1366MomentaryInterruptionEvent"@en .


#-- ieee1366SAIDI
eme:ieee1366SAIDI rdf:type owl:NamedIndividual ,
                           eme:MeasurementKind ;
                  rdfs:label "ieee1366SAIDI"@en .


#-- ieee1366SAIFI
eme:ieee1366SAIFI rdf:type owl:NamedIndividual ,
                           eme:MeasurementKind ;
                  rdfs:label "ieee1366SAIFI"@en .


#-- ieee1366SustainedInterruption
eme:ieee1366SustainedInterruption rdf:type owl:NamedIndividual ,
                                           eme:MeasurementKind ;
                                  rdfs:label "ieee1366SustainedInterruption"@en .


#-- indicating
eme:indicating rdf:type owl:NamedIndividual ,
                        eme:AccumulationKind ;
               rdfs:comment """As if a needle is swung out on the meter face to a value to indicate the current value.
Note: An 'indicating' value is typically measured over hundreds of milliseconds or greater, or may imply a “pusher” mechanism to capture a value. Compare this to 'instantaneous' which is measured over a shorter period of time."""@en .


#-- instantaneous
eme:instantaneous rdf:type owl:NamedIndividual ,
                           eme:AccumulationKind ;
                  rdfs:comment """Typically measured over the fastest period of time allowed by the definition of the metric (usually milliseconds or tens of milliseconds.)
Note: 'instantaneous' was moved to attribute #3 in Ed.2 of IEC 61968-9, from attribute #1 in Ed.1 of IEC 61968-9."""@en .


#-- insulativeGas
eme:insulativeGas rdf:type owl:NamedIndividual ,
                           eme:CommodityKind .


#-- insulativeOil
eme:insulativeOil rdf:type owl:NamedIndividual ,
                           eme:CommodityKind .


#-- internalUse
eme:internalUse rdf:type owl:NamedIndividual ,
                         eme:CustomerKind ;
                rdfs:comment "Internal use customer."@en .


#-- internet
eme:internet rdf:type owl:NamedIndividual ,
                      eme:CommodityKind ;
             rdfs:comment "Internet service"@en .


#-- interruptionBehaviour
eme:interruptionBehaviour rdf:type owl:NamedIndividual ,
                                   eme:MeasurementKind ;
                          rdfs:label "interruptionBehaviour"@en .


#-- inversionTamper
eme:inversionTamper rdf:type owl:NamedIndividual ,
                             eme:MeasurementKind ;
                    rdfs:label "inversionTamper"@en .


#-- ipAddress
eme:ipAddress rdf:type owl:NamedIndividual ,
                       eme:MeasurementKind ;
              rdfs:label "ipAddress"@en .


#-- k
eme:k rdf:type owl:NamedIndividual ,
               eme:UnitMultiplier ;
      rdfs:comment "Kilo 103." ;
      rdfs:label "k"@en .


#-- kat
eme:kat rdf:type owl:NamedIndividual ,
                 eme:UnitSymbol ;
        rdfs:comment "Catalytic activity katal  mol  s." ;
        rdfs:label "kat"@en .


#-- katPerm3
eme:katPerm3 rdf:type owl:NamedIndividual ,
                      eme:UnitSymbol ;
             rdfs:comment "Catalytic activity concentration katals per cubic metre." ;
             rdfs:label "katPerm3"@en .


#-- kg
eme:kg rdf:type owl:NamedIndividual ,
                eme:UnitSymbol ;
       rdfs:comment "Mass in kilograms.  Note multiplier k is included in this unit symbol for compatibility with IEC 6185073." ;
       rdfs:label "kg"@en .


#-- kgPerJ
eme:kgPerJ rdf:type owl:NamedIndividual ,
                    eme:UnitSymbol ;
           rdfs:comment "Weight per energy in kilograms per joule kgJ. Note multiplier k is included in this unit symbol for compatibility with IEC 6185073." ;
           rdfs:label "kgPerJ"@en .


#-- kgPerm3
eme:kgPerm3 rdf:type owl:NamedIndividual ,
                     eme:UnitSymbol ;
            rdfs:comment "Density in kilogramcubic metres kgm. Note multiplier k is included in this unit symbol for compatibility with IEC 6185073." ;
            rdfs:label "kgPerm3"@en .


#-- kgm
eme:kgm rdf:type owl:NamedIndividual ,
                 eme:UnitSymbol ;
        rdfs:comment "Moment of mass in kilogram metres kgm first moment of mass. Note multiplier k is included in this unit symbol for compatibility with IEC 6185073." ;
        rdfs:label "kgm"@en .


#-- kgm2
eme:kgm2 rdf:type owl:NamedIndividual ,
                  eme:UnitSymbol ;
         rdfs:comment "Moment of mass in kilogram square metres kgm Second moment of mass commonly called the moment of inertia. Note multiplier k is included in this unit symbol for compatibility with IEC 6185073." ;
         rdfs:label "kgm2"@en .


#-- kn
eme:kn rdf:type owl:NamedIndividual ,
                eme:UnitSymbol ;
       rdfs:comment "Speed knots 1 kn  18523600 ms." ;
       rdfs:label "kn"@en .


#-- l
eme:l rdf:type owl:NamedIndividual ,
               eme:UnitSymbol ;
      rdfs:comment "Volume in litres litre  dm3  m31000." ;
      rdfs:label "l"@en .


#-- lPerh
eme:lPerh rdf:type owl:NamedIndividual ,
                   eme:UnitSymbol ;
          rdfs:comment "Volumetric flow rate litres per hour." ;
          rdfs:label "lPerh"@en .


#-- lPerl
eme:lPerl rdf:type owl:NamedIndividual ,
                   eme:UnitSymbol ;
          rdfs:comment "Concentration The ratio of the volume of a solute divided by the volume of  the solution. Note Users may need use a prefix such a  to express a quantity such as LL." ;
          rdfs:label "lPerl"@en .


#-- lPers
eme:lPers rdf:type owl:NamedIndividual ,
                   eme:UnitSymbol ;
          rdfs:comment "Volumetric flow rate in litres per second." ;
          rdfs:label "lPers"@en .


#-- lagging
eme:lagging rdf:type owl:NamedIndividual ,
                     eme:FlowDirectionKind ;
            rdfs:comment """Typically used to describe that a power factor is lagging the reference value. 
Note 1: When used to describe VA, “lagging” describes a form of measurement where reactive power is considered in all four quadrants, but real power is considered only in quadrants I and IV.
Note 2: When used to describe power factor, the term “Lagging” implies that the PF is negative. The term “lagging” in this case takes the place of the negative sign. If a signed PF value is to be passed by the data producer, then the direction of flow enumeration zero (none) should be used in order to avoid the possibility of creating an expression that employs a double negative. The data consumer should be able to tell from the sign of the data if the PF is leading or lagging. This principle is analogous to the concept that “Reverse” energy is an implied negative value, and to publish a negative reverse value would be ambiguous.
Note 3: Lagging power factors typically indicate inductive loading."""@en .


#-- latchingQuantity
eme:latchingQuantity rdf:type owl:NamedIndividual ,
                              eme:AccumulationKind ;
                     rdfs:comment """When this description is applied to a metered value, it implies that the value is a time-independent cumulative quantity much like a 'bulkQuantity', except that it latches upon the maximum value upon reaching that value. Any additional accumulation (positive or negative) is discarded until a reset occurs. 
Note: A 'latchingQuantity' may also occur in the downward direction – upon reaching a minimum value. The terms 'maximum' or 'minimum' (for 'aggregate') will usually be included when this type of accumulation behaviour is present. 
When this description is applied to an encoded value (UOM= 'Code'), it implies that the value has one or more bits which are latching. The condition that caused the bit to be set may have long since evaporated.
In either case, the timestamp that accompanies the value may not coincide with the moment the value was initially set.
In both cases a system will need to perform an operation to clear the latched value."""@en .


#-- leading
eme:leading rdf:type owl:NamedIndividual ,
                     eme:FlowDirectionKind ;
            rdfs:comment """Typically used to describe that a power factor is leading the reference value.
Note: Leading power factors typically indicate capacitive loading."""@en .


#-- lineLoss
eme:lineLoss rdf:type owl:NamedIndividual ,
                      eme:MeasurementKind ;
             rdfs:label "lineLoss"@en .


#-- lm
eme:lm rdf:type owl:NamedIndividual ,
                eme:UnitSymbol ;
       rdfs:comment "Luminous flux in lumens cdsr." ;
       rdfs:label "lm"@en .


#-- loadInterrupt
eme:loadInterrupt rdf:type owl:NamedIndividual ,
                           eme:MeasurementKind ;
                  rdfs:label "loadInterrupt"@en .


#-- loadShed
eme:loadShed rdf:type owl:NamedIndividual ,
                      eme:MeasurementKind ;
             rdfs:label "loadShed"@en .


#-- loss
eme:loss rdf:type owl:NamedIndividual ,
                  eme:MeasurementKind ;
         rdfs:label "loss"@en .


#-- lowThreshold
eme:lowThreshold rdf:type owl:NamedIndividual ,
                          eme:AggregateKind ;
                 rdfs:comment "The value represents a programmed low threshold."@en .


#-- lx
eme:lx rdf:type owl:NamedIndividual ,
                eme:UnitSymbol ;
       rdfs:comment "Illuminance in lux lmm." ;
       rdfs:label "lx"@en .


#-- m
eme:m rdf:type owl:NamedIndividual ,
               eme:UnitMultiplier ,
               eme:UnitSymbol ;
      rdfs:comment "Length in metres." ,
                   "Milli 103." ;
      rdfs:label "m"@en .


#-- m2
eme:m2 rdf:type owl:NamedIndividual ,
                eme:UnitSymbol ;
       rdfs:comment "Area in square metres m." ;
       rdfs:label "m2"@en .


#-- m2Pers
eme:m2Pers rdf:type owl:NamedIndividual ,
                    eme:UnitSymbol ;
           rdfs:comment "Viscosity in square metres  second ms." ;
           rdfs:label "m2Pers"@en .


#-- m3
eme:m3 rdf:type owl:NamedIndividual ,
                eme:UnitSymbol ;
       rdfs:comment "Volume in cubic metres m." ;
       rdfs:label "m3"@en .


#-- m3Compensated
eme:m3Compensated rdf:type owl:NamedIndividual ,
                           eme:UnitSymbol ;
                  rdfs:comment "Volume cubic metres with the value compensated for weather effects." ;
                  rdfs:label "m3Compensated"@en .


#-- m3Perh
eme:m3Perh rdf:type owl:NamedIndividual ,
                    eme:UnitSymbol ;
           rdfs:comment "Volumetric flow rate cubic metres per hour." ;
           rdfs:label "m3Perh"@en .


#-- m3Perkg
eme:m3Perkg rdf:type owl:NamedIndividual ,
                     eme:UnitSymbol ;
            rdfs:comment "Specific volume cubic metres per kilogram v." ;
            rdfs:label "m3Perkg"@en .


#-- m3Pers
eme:m3Pers rdf:type owl:NamedIndividual ,
                    eme:UnitSymbol ;
           rdfs:comment "Volumetric flow rate in cubic metres per second ms." ;
           rdfs:label "m3Pers"@en .


#-- m3Uncompensated
eme:m3Uncompensated rdf:type owl:NamedIndividual ,
                             eme:UnitSymbol ;
                    rdfs:comment "Volume cubic metres with the value uncompensated for weather effects." ;
                    rdfs:label "m3Uncompensated"@en .


#-- mPerm3
eme:mPerm3 rdf:type owl:NamedIndividual ,
                    eme:UnitSymbol ;
           rdfs:comment "Fuel efficiency in metres per cubic metres mm." ;
           rdfs:label "mPerm3"@en .


#-- mPers
eme:mPers rdf:type owl:NamedIndividual ,
                   eme:UnitSymbol ;
          rdfs:comment "Velocity in metres per second ms." ;
          rdfs:label "mPers"@en .


#-- mPers2
eme:mPers2 rdf:type owl:NamedIndividual ,
                    eme:UnitSymbol ;
           rdfs:comment "Acceleration in metres per second squared ms." ;
           rdfs:label "mPers2"@en .


#-- macAddress
eme:macAddress rdf:type owl:NamedIndividual ,
                        eme:MeasurementKind ;
               rdfs:label "macAddress"@en .


#-- maintenance
eme:maintenance rdf:type owl:NamedIndividual ,
                         eme:MeasurementKind ;
                rdfs:label "maintenance"@en .


#-- maximum
eme:maximum rdf:type owl:NamedIndividual ,
                     eme:AggregateKind ;
            rdfs:comment "The highest value observed."@en .


#-- mfgAssignedConfigurationID
eme:mfgAssignedConfigurationID rdf:type owl:NamedIndividual ,
                                        eme:MeasurementKind ;
                               rdfs:label "mfgAssignedConfigurationID"@en .


#-- mfgAssignedPhysicalSerialNumber
eme:mfgAssignedPhysicalSerialNumber rdf:type owl:NamedIndividual ,
                                             eme:MeasurementKind ;
                                    rdfs:label "mfgAssignedPhysicalSerialNumber"@en .


#-- mfgAssignedProductNumber
eme:mfgAssignedProductNumber rdf:type owl:NamedIndividual ,
                                      eme:MeasurementKind ;
                             rdfs:label "mfgAssignedProductNumber"@en .


#-- mfgAssignedUniqueCommunicationAddress
eme:mfgAssignedUniqueCommunicationAddress rdf:type owl:NamedIndividual ,
                                                   eme:MeasurementKind ;
                                          rdfs:label "mfgAssignedUniqueCommunicationAddress"@en .


#-- micro
eme:micro rdf:type owl:NamedIndividual ,
                   eme:UnitMultiplier ;
          rdfs:comment "Micro 106." ;
          rdfs:label "micro"@en .


#-- min
eme:min rdf:type owl:NamedIndividual ,
                 eme:UnitSymbol ;
        rdfs:comment "Time in minutes minute   60 s." ;
        rdfs:label "min"@en .


#-- minimum
eme:minimum rdf:type owl:NamedIndividual ,
                     eme:AggregateKind ;
            rdfs:comment "The smallest value observed."@en .


#-- mmHg
eme:mmHg rdf:type owl:NamedIndividual ,
                  eme:UnitSymbol ;
         rdfs:comment "Pressure millimetres of mercury 1 mmHg is approximately 133.3 Pa." ;
         rdfs:label "mmHg"@en .


#-- mol
eme:mol rdf:type owl:NamedIndividual ,
                 eme:UnitSymbol ;
        rdfs:comment "Amount of substance in moles." ;
        rdfs:label "mol"@en .


#-- molPerkg
eme:molPerkg rdf:type owl:NamedIndividual ,
                      eme:UnitSymbol ;
             rdfs:comment "Concentration Molality the amount of solute in moles and the amount of solvent in kilograms." ;
             rdfs:label "molPerkg"@en .


#-- molPerm3
eme:molPerm3 rdf:type owl:NamedIndividual ,
                      eme:UnitSymbol ;
             rdfs:comment "Concentration The amount of substance concentration c the amount of solvent in moles divided by the volume of solution in m." ;
             rdfs:label "molPerm3"@en .


#-- molPermol
eme:molPermol rdf:type owl:NamedIndividual ,
                       eme:UnitSymbol ;
              rdfs:comment "Concentration Molar fraction the ratio of the molar amount of a solute divided by the molar amount of the solution." ;
              rdfs:label "molPermol"@en .


#-- monthly
eme:monthly rdf:type owl:NamedIndividual ,
                     eme:MacroPeriodKind ;
            rdfs:comment "Monthly period starting at midnight on the first day of the month. If within the current month, this specifies the period from the start of the month until \"now.\""@en .


#-- multiCastAddress
eme:multiCastAddress rdf:type owl:NamedIndividual ,
                              eme:MeasurementKind ;
                     rdfs:label "multiCastAddress"@en .


#-- n
eme:n rdf:type owl:NamedIndividual ,
               eme:UnitMultiplier ;
      rdfs:comment "Nano 109." ;
      rdfs:label "n"@en .


#-- naturalGas
eme:naturalGas rdf:type owl:NamedIndividual ,
                        eme:CommodityKind .


#-- negativeSequence
eme:negativeSequence rdf:type owl:NamedIndividual ,
                              eme:MeasurementKind ;
                     rdfs:label "negativeSequence"@en .


#-- net
eme:net rdf:type owl:NamedIndividual ,
                 eme:FlowDirectionKind ;
        rdfs:comment """|Forward| - |Reverse|, See 61968-2.

Note: In some systems, the value passed as a “net” value could become negative. In other systems the value passed as a “net” value is always a positive number, and rolls-over and rolls-under as needed."""@en .


#-- nominal
eme:nominal rdf:type owl:NamedIndividual ,
                     eme:AggregateKind ;
            rdfs:comment "The nominal value."@en .


#-- none
eme:none rdf:type owl:NamedIndividual ,
                  [ rdf:type owl:Class ;
                    owl:unionOf ( eme:AccumulationKind
                  eme:AggregateKind
                  eme:CommodityKind
                  eme:FlowDirectionKind
                  eme:MacroPeriodKind
                  eme:MeasurementKind
                  eme:MeasuringPeriodKind
                  eme:UnitMultiplier
                  eme:UnitSymbol
                                )
                  ] ;
         rdfs:comment """(AccumulationKind) Not applicable, or implied by the unit of measure. 
(UnitSymbol) Dimension less quantity e.g. count per unit etc.
(UnitMultiplier) No multiplier or equivalently multiply by 1. 
(AggregateKind, CommodityKind, FlowDirectionKind, MacroPeriodKind, MeasurementKind, MeasuringPeriodKind) Not Applicable.""" @en ;
         rdfs:label "none"@en .


#-- nonpotableWater
eme:nonpotableWater rdf:type owl:NamedIndividual ,
                             eme:CommodityKind ;
                    rdfs:comment "Reclaimed water – possibly used for irrigation but not sufficiently treated to be considered safe for drinking."@en .


#-- normal
eme:normal rdf:type owl:NamedIndividual ,
                    eme:AggregateKind ;
           rdfs:comment "The normal value."@en .


#-- nox
eme:nox rdf:type owl:NamedIndividual ,
                 eme:CommodityKind ;
        rdfs:comment "Nitrous Oxides NOX"@en .


#-- ohm
eme:ohm rdf:type owl:NamedIndividual ,
                 eme:UnitSymbol ;
        rdfs:comment "Electric resistance in ohms VA." ;
        rdfs:label "ohm"@en .


#-- ohmPerm
eme:ohmPerm rdf:type owl:NamedIndividual ,
                     eme:UnitSymbol ;
            rdfs:comment "Electric resistance per length in ohms per metre VAm." ;
            rdfs:label "ohmPerm"@en .


#-- ohmm
eme:ohmm rdf:type owl:NamedIndividual ,
                  eme:UnitSymbol ;
         rdfs:comment "Resistivity ohm metres rho." ;
         rdfs:label "ohmm"@en .


#-- oneMinute
eme:oneMinute rdf:type owl:NamedIndividual ,
                       eme:MeasuringPeriodKind ;
              rdfs:comment "1-minute"@en .


#-- onePerHz
eme:onePerHz rdf:type owl:NamedIndividual ,
                      eme:UnitSymbol ;
             rdfs:comment "Reciprocal of frequency 1Hz." ;
             rdfs:label "onePerHz"@en .


#-- onePerm
eme:onePerm rdf:type owl:NamedIndividual ,
                     eme:UnitSymbol ;
            rdfs:comment "Wavenumber reciprocal metres  1m." ;
            rdfs:label "onePerm"@en .


#-- oneWayAddress
eme:oneWayAddress rdf:type owl:NamedIndividual ,
                           eme:MeasurementKind ;
                  rdfs:label "oneWayAddress"@en .


#-- other
eme:other rdf:type owl:NamedIndividual ,
                   eme:CustomerKind ;
          rdfs:comment "Other kind of customer."@en .


#-- p
eme:p rdf:type owl:NamedIndividual ,
               eme:UnitMultiplier ;
      rdfs:comment "Pico 1012." ;
      rdfs:label "p"@en .


#-- pfc
eme:pfc rdf:type owl:NamedIndividual ,
                 eme:CommodityKind ;
        rdfs:comment "Perfluorocarbons PFC"@en .


#-- phasorPowerFactor
eme:phasorPowerFactor rdf:type owl:NamedIndividual ,
                               eme:MeasurementKind ;
                      rdfs:label "phasorPowerFactor"@en .


#-- phasorReactivePower
eme:phasorReactivePower rdf:type owl:NamedIndividual ,
                                 eme:MeasurementKind ;
                        rdfs:label "phasorReactivePower"@en .


#-- physicalTamper
eme:physicalTamper rdf:type owl:NamedIndividual ,
                            eme:MeasurementKind ;
                   rdfs:label "physicalTamper"@en .


#-- positiveSequence
eme:positiveSequence rdf:type owl:NamedIndividual ,
                              eme:MeasurementKind ;
                     rdfs:label "positiveSequence"@en .


#-- potableWater
eme:potableWater rdf:type owl:NamedIndividual ,
                          eme:CommodityKind ;
                 rdfs:comment "Drinkable water"@en .


#-- power
eme:power rdf:type owl:NamedIndividual ,
                   eme:MeasurementKind ;
          rdfs:label "power"@en .


#-- powerFactor
eme:powerFactor rdf:type owl:NamedIndividual ,
                         eme:MeasurementKind ;
                rdfs:label "powerFactor"@en .


#-- powerLossTamper
eme:powerLossTamper rdf:type owl:NamedIndividual ,
                             eme:MeasurementKind ;
                    rdfs:label "powerLossTamper"@en .


#-- powerOutage
eme:powerOutage rdf:type owl:NamedIndividual ,
                         eme:MeasurementKind ;
                rdfs:label "powerOutage"@en .


#-- powerQuality
eme:powerQuality rdf:type owl:NamedIndividual ,
                          eme:MeasurementKind ;
                 rdfs:label "powerQuality"@en .


#-- powerRestoration
eme:powerRestoration rdf:type owl:NamedIndividual ,
                              eme:MeasurementKind ;
                     rdfs:label "powerRestoration"@en .


#-- ppm
eme:ppm rdf:type owl:NamedIndividual ,
                 eme:UnitSymbol ;
        rdfs:comment "Concentration in parts per million." ;
        rdfs:label "ppm"@en .


#-- present
eme:present rdf:type owl:NamedIndividual ,
                     eme:MeasuringPeriodKind ;
            rdfs:comment "Within the present period of time"@en .


#-- previous
eme:previous rdf:type owl:NamedIndividual ,
                      eme:MeasuringPeriodKind ;
             rdfs:comment "Shifted within the previous monthly cycle and data set"@en .


#-- programmed
eme:programmed rdf:type owl:NamedIndividual ,
                        eme:MeasurementKind ;
               rdfs:label "programmed"@en .


#-- propane
eme:propane rdf:type owl:NamedIndividual ,
                     eme:CommodityKind .


#-- pumpingLoad
eme:pumpingLoad rdf:type owl:NamedIndividual ,
                         eme:CustomerKind ;
                rdfs:comment "Pumping load customer."@en .


#-- pushbutton
eme:pushbutton rdf:type owl:NamedIndividual ,
                        eme:MeasurementKind ;
               rdfs:label "pushbutton"@en .


#-- q1minusQ4
eme:q1minusQ4 rdf:type owl:NamedIndividual ,
                       eme:FlowDirectionKind ;
              rdfs:comment "Q1 minus Q4"@en .


#-- q1plusQ2
eme:q1plusQ2 rdf:type owl:NamedIndividual ,
                      eme:FlowDirectionKind ;
             rdfs:comment "Reactive positive quadrants. (The term “lagging” is preferred.)"@en .


#-- q1plusQ3
eme:q1plusQ3 rdf:type owl:NamedIndividual ,
                      eme:FlowDirectionKind ;
             rdfs:comment "Quadrants 1 and 3"@en .


#-- q1plusQ4
eme:q1plusQ4 rdf:type owl:NamedIndividual ,
                      eme:FlowDirectionKind ;
             rdfs:comment "Quadrants 1 and 4 usually represent forward active energy"@en .


#-- q2minusQ3
eme:q2minusQ3 rdf:type owl:NamedIndividual ,
                       eme:FlowDirectionKind ;
              rdfs:comment "Q2 minus Q3"@en .


#-- q2plusQ3
eme:q2plusQ3 rdf:type owl:NamedIndividual ,
                      eme:FlowDirectionKind ;
             rdfs:comment "Quadrants 2 and 3 usually represent reverse active energy"@en .


#-- q2plusQ4
eme:q2plusQ4 rdf:type owl:NamedIndividual ,
                      eme:FlowDirectionKind ;
             rdfs:comment "Quadrants 2 and 4"@en .


#-- q3minusQ2
eme:q3minusQ2 rdf:type owl:NamedIndividual ,
                       eme:FlowDirectionKind ;
              rdfs:comment "Q3 minus Q2"@en .


#-- q3plusQ4
eme:q3plusQ4 rdf:type owl:NamedIndividual ,
                      eme:FlowDirectionKind ;
             rdfs:comment "Reactive negative quadrants. (The term “leading” is preferred.)"@en .


#-- quadrant1
eme:quadrant1 rdf:type owl:NamedIndividual ,
                       eme:FlowDirectionKind ;
              rdfs:comment "Q1 only"@en .


#-- quadrant2
eme:quadrant2 rdf:type owl:NamedIndividual ,
                       eme:FlowDirectionKind ;
              rdfs:comment "Q2 only"@en .


#-- quadrant3
eme:quadrant3 rdf:type owl:NamedIndividual ,
                       eme:FlowDirectionKind ;
              rdfs:comment "Q3 only"@en .


#-- quadrant4
eme:quadrant4 rdf:type owl:NamedIndividual ,
                       eme:FlowDirectionKind ;
              rdfs:comment "Q4 only"@en .


#-- quantityPower
eme:quantityPower rdf:type owl:NamedIndividual ,
                           eme:MeasurementKind ;
                  rdfs:label "quantityPower"@en .


#-- rad
eme:rad rdf:type owl:NamedIndividual ,
                 eme:UnitSymbol ;
        rdfs:comment "Plane angle in radians mm." ;
        rdfs:label "rad"@en .


#-- radPers
eme:radPers rdf:type owl:NamedIndividual ,
                     eme:UnitSymbol ;
            rdfs:comment "Angular velocity in radians per second rads." ;
            rdfs:label "radPers"@en .


#-- radPers2
eme:radPers2 rdf:type owl:NamedIndividual ,
                      eme:UnitSymbol ;
             rdfs:comment "Angular acceleration radians per second squared." ;
             rdfs:label "radPers2"@en .


#-- refuse
eme:refuse rdf:type owl:NamedIndividual ,
                    eme:CommodityKind ;
           rdfs:comment "trash"@en .


#-- relayActivation
eme:relayActivation rdf:type owl:NamedIndividual ,
                             eme:MeasurementKind ;
                    rdfs:label "relayActivation"@en .


#-- relayCycle
eme:relayCycle rdf:type owl:NamedIndividual ,
                        eme:MeasurementKind ;
               rdfs:comment "Usually expressed as a count" ;
               rdfs:label "relayCycle"@en .


#-- removalTamper
eme:removalTamper rdf:type owl:NamedIndividual ,
                           eme:MeasurementKind ;
                  rdfs:label "removalTamper"@en .


#-- reprogrammingTamper
eme:reprogrammingTamper rdf:type owl:NamedIndividual ,
                                 eme:MeasurementKind ;
                        rdfs:label "reprogrammingTamper"@en .


#-- residential
eme:residential rdf:type owl:NamedIndividual ,
                         eme:CustomerKind ;
                rdfs:comment "Residential customer."@en .


#-- residentialAndCommercial
eme:residentialAndCommercial rdf:type owl:NamedIndividual ,
                                      eme:CustomerKind ;
                             rdfs:comment "Residential and commercial customer."@en .


#-- residentialAndStreetlight
eme:residentialAndStreetlight rdf:type owl:NamedIndividual ,
                                       eme:CustomerKind ;
                              rdfs:comment "Residential and streetlight customer."@en .


#-- residentialFarmService
eme:residentialFarmService rdf:type owl:NamedIndividual ,
                                    eme:CustomerKind ;
                           rdfs:comment "Residential farm service customer."@en .


#-- residentialStreetlightOthers
eme:residentialStreetlightOthers rdf:type owl:NamedIndividual ,
                                          eme:CustomerKind ;
                                 rdfs:comment "Residential streetlight or other related customer."@en .


#-- rev
eme:rev rdf:type owl:NamedIndividual ,
                 eme:UnitSymbol ;
        rdfs:comment "Amount of rotation revolutions." ;
        rdfs:label "rev"@en .


#-- reverse
eme:reverse rdf:type owl:NamedIndividual ,
                     eme:FlowDirectionKind ;
            rdfs:comment """Reverse Active Energy is equivalent to \"Received,\" or \"Exported\" as defined in 61968-2.
Reverse Active Energy is a positive kWh value as one would expect to find when energy is backfed by the service onto the utility network.
Reverse Reactive Energy is a positive VArh value as one would expect to find in the presence of capacitive loading and a leading Power Factor.
In polyphase metering, the reverse energy register is incremented when the sum of the phase energies is less than zero:
<img src=\"HTS_1.PNG\" width=\"209\" height=\"16\" border=\"0\" alt=\"graphic\"/>
Note: The value passed as a reverse value is always a positive value. It is understood by the label “reverse” that it represents negative flow."""@en .


#-- reverseRotationTamper
eme:reverseRotationTamper rdf:type owl:NamedIndividual ,
                                   eme:MeasurementKind ;
                          rdfs:label "reverseRotationTamper"@en .


#-- rollingBlock10MinIntvl1MinSubIntvl
eme:rollingBlock10MinIntvl1MinSubIntvl rdf:type owl:NamedIndividual ,
                                                eme:MeasuringPeriodKind ;
                                       rdfs:comment "10-minute Rolling Block with 1-minute sub-intervals"@en .


#-- rollingBlock10MinIntvl2MinSubIntvl
eme:rollingBlock10MinIntvl2MinSubIntvl rdf:type owl:NamedIndividual ,
                                                eme:MeasuringPeriodKind ;
                                       rdfs:comment "10-minute Rolling Block with 2-minute sub-intervals"@en .


#-- rollingBlock10MinIntvl5MinSubIntvl
eme:rollingBlock10MinIntvl5MinSubIntvl rdf:type owl:NamedIndividual ,
                                                eme:MeasuringPeriodKind ;
                                       rdfs:comment "10-minute Rolling Block with 5-minute sub-intervals"@en .


#-- rollingBlock15MinIntvl1MinSubIntvl
eme:rollingBlock15MinIntvl1MinSubIntvl rdf:type owl:NamedIndividual ,
                                                eme:MeasuringPeriodKind ;
                                       rdfs:comment "15-minute Rolling Block with 1-minute sub-intervals"@en .


#-- rollingBlock15MinIntvl3MinSubIntvl
eme:rollingBlock15MinIntvl3MinSubIntvl rdf:type owl:NamedIndividual ,
                                                eme:MeasuringPeriodKind ;
                                       rdfs:comment "15-minute Rolling Block with 3-minute sub-intervals"@en .


#-- rollingBlock15MinIntvl5MinSubIntvl
eme:rollingBlock15MinIntvl5MinSubIntvl rdf:type owl:NamedIndividual ,
                                                eme:MeasuringPeriodKind ;
                                       rdfs:comment "15-minute Rolling Block with 5-minute sub-intervals"@en .


#-- rollingBlock30MinIntvl10MinSubIntvl
eme:rollingBlock30MinIntvl10MinSubIntvl rdf:type owl:NamedIndividual ,
                                                 eme:MeasuringPeriodKind ;
                                        rdfs:comment "30-minute Rolling Block with 10-minute sub-intervals"@en .


#-- rollingBlock30MinIntvl15MinSubIntvl
eme:rollingBlock30MinIntvl15MinSubIntvl rdf:type owl:NamedIndividual ,
                                                 eme:MeasuringPeriodKind ;
                                        rdfs:comment "30-minute Rolling Block with 15-minute sub-intervals"@en .


#-- rollingBlock30MinIntvl2MinSubIntvl
eme:rollingBlock30MinIntvl2MinSubIntvl rdf:type owl:NamedIndividual ,
                                                eme:MeasuringPeriodKind ;
                                       rdfs:comment "30-minute Rolling Block with 2-minute sub-intervals"@en .


#-- rollingBlock30MinIntvl3MinSubIntvl
eme:rollingBlock30MinIntvl3MinSubIntvl rdf:type owl:NamedIndividual ,
                                                eme:MeasuringPeriodKind ;
                                       rdfs:comment "30-minute Rolling Block with 3-minute sub-intervals"@en .


#-- rollingBlock30MinIntvl5MinSubIntvl
eme:rollingBlock30MinIntvl5MinSubIntvl rdf:type owl:NamedIndividual ,
                                                eme:MeasuringPeriodKind ;
                                       rdfs:comment "30-minute Rolling Block with 5-minute sub-intervals."@en .


#-- rollingBlock30MinIntvl6MinSubIntvl
eme:rollingBlock30MinIntvl6MinSubIntvl rdf:type owl:NamedIndividual ,
                                                eme:MeasuringPeriodKind ;
                                       rdfs:comment "30-minute Rolling Block with 6-minute sub-intervals"@en .


#-- rollingBlock5MinIntvl1MinSubIntvl
eme:rollingBlock5MinIntvl1MinSubIntvl rdf:type owl:NamedIndividual ,
                                               eme:MeasuringPeriodKind ;
                                      rdfs:comment "5-minute Rolling Block with 1-minute sub-intervals"@en .


#-- rollingBlock60MinIntvl10MinSubIntvl
eme:rollingBlock60MinIntvl10MinSubIntvl rdf:type owl:NamedIndividual ,
                                                 eme:MeasuringPeriodKind ;
                                        rdfs:comment "60-minute Rolling Block with 10-minute sub-intervals"@en .


#-- rollingBlock60MinIntvl12MinSubIntvl
eme:rollingBlock60MinIntvl12MinSubIntvl rdf:type owl:NamedIndividual ,
                                                 eme:MeasuringPeriodKind ;
                                        rdfs:comment "60-minute Rolling Block with 12-minute sub-intervals"@en .


#-- rollingBlock60MinIntvl15MinSubIntvl
eme:rollingBlock60MinIntvl15MinSubIntvl rdf:type owl:NamedIndividual ,
                                                 eme:MeasuringPeriodKind ;
                                        rdfs:comment "60-minute Rolling Block with 15-minute sub-intervals"@en .


#-- rollingBlock60MinIntvl20MinSubIntvl
eme:rollingBlock60MinIntvl20MinSubIntvl rdf:type owl:NamedIndividual ,
                                                 eme:MeasuringPeriodKind ;
                                        rdfs:comment "60-minute Rolling Block with 20-minute sub-intervals"@en .


#-- rollingBlock60MinIntvl30MinSubIntvl
eme:rollingBlock60MinIntvl30MinSubIntvl rdf:type owl:NamedIndividual ,
                                                 eme:MeasuringPeriodKind ;
                                        rdfs:comment "60-minute Rolling Block with 30-minute sub-intervals" .


#-- rollingBlock60MinIntvl4MinSubIntvl
eme:rollingBlock60MinIntvl4MinSubIntvl rdf:type owl:NamedIndividual ,
                                                eme:MeasuringPeriodKind ;
                                       rdfs:comment "60-minute Rolling Block with 4-minute sub-intervals"@en .


#-- rollingBlock60MinIntvl5MinSubIntvl
eme:rollingBlock60MinIntvl5MinSubIntvl rdf:type owl:NamedIndividual ,
                                                eme:MeasuringPeriodKind ;
                                       rdfs:comment "60-minute Rolling Block with 5-minute sub-intervals"@en .


#-- rollingBlock60MinIntvl6MinSubIntvl
eme:rollingBlock60MinIntvl6MinSubIntvl rdf:type owl:NamedIndividual ,
                                                eme:MeasuringPeriodKind ;
                                       rdfs:comment "60-minute Rolling Block with 6-minute sub-intervals"@en .


#-- rotPers
eme:rotPers rdf:type owl:NamedIndividual ,
                     eme:UnitSymbol ;
            rdfs:comment "Rotations per second 1s. See also Hz 1s." ;
            rdfs:label "rotPers"@en .


#-- s
eme:s rdf:type owl:NamedIndividual ,
               eme:UnitSymbol ;
      rdfs:comment "Time in seconds." ;
      rdfs:label "s"@en .


#-- s1
eme:s1 rdf:type owl:NamedIndividual ,
                eme:PhaseCode ;
       rdfs:comment "Secondary phase 1."@en .


#-- s12
eme:s12 rdf:type owl:NamedIndividual ,
                 eme:PhaseCode ;
        rdfs:comment "Secondary phase 1 and 2."@en .


#-- s12N
eme:s12N rdf:type owl:NamedIndividual ,
                  eme:PhaseCode ;
         rdfs:comment "Secondary phases 1, 2, and neutral."@en .


#-- s1N
eme:s1N rdf:type owl:NamedIndividual ,
                 eme:PhaseCode ;
        rdfs:comment "Secondary phase 1 and neutral."@en .


#-- s2
eme:s2 rdf:type owl:NamedIndividual ,
                eme:PhaseCode ;
       rdfs:comment "Secondary phase 2."@en .


#-- s2N
eme:s2N rdf:type owl:NamedIndividual ,
                 eme:PhaseCode ;
        rdfs:comment "Secondary phase 2 and neutral."@en .


#-- sPers
eme:sPers rdf:type owl:NamedIndividual ,
                   eme:UnitSymbol ;
          rdfs:comment "Time Ratio of time.  Note Users may need to supply a prefix such as 181 to show rates such as 181ss." ;
          rdfs:label "sPers"@en .


#-- sag
eme:sag rdf:type owl:NamedIndividual ,
                 eme:MeasurementKind ;
        rdfs:comment "or Voltage Dip" ;
        rdfs:label "sag"@en .


#-- seasonal
eme:seasonal rdf:type owl:NamedIndividual ,
                      eme:MacroPeriodKind ;
             rdfs:comment "A season of time spanning multiple months. E.g. \"Summer,\" \"Spring,\" \"Fall,\" and \"Winter\" based cycle. If within the current season, it specifies the period from the start of the current season until \"now.\""@en .


#-- secondMaximum
eme:secondMaximum rdf:type owl:NamedIndividual ,
                           eme:AggregateKind ;
                  rdfs:comment "The second highest value observed."@en .


#-- secondMinimum
eme:secondMinimum rdf:type owl:NamedIndividual ,
                           eme:AggregateKind ;
                  rdfs:comment "The second smallest value observed."@en .


#-- sf6
eme:sf6 rdf:type owl:NamedIndividual ,
                 eme:CommodityKind ;
        rdfs:comment "Sulfurhexafluoride SF6"@en .


#-- signalStrength
eme:signalStrength rdf:type owl:NamedIndividual ,
                            eme:MeasurementKind ;
                   rdfs:label "signalStrength"@en .


#-- signaltoNoiseRatio
eme:signaltoNoiseRatio rdf:type owl:NamedIndividual ,
                                eme:MeasurementKind ;
                       rdfs:comment "Moved here from Attribute 9 UOM" ;
                       rdfs:label "signaltoNoiseRatio"@en .


#-- sixtyMinute
eme:sixtyMinute rdf:type owl:NamedIndividual ,
                         eme:MeasuringPeriodKind ;
                rdfs:comment "60-minute"@en .


#-- so2
eme:so2 rdf:type owl:NamedIndividual ,
                 eme:CommodityKind ;
        rdfs:comment "Sulfur Dioxide SO2"@en .


#-- specifiedPeriod
eme:specifiedPeriod rdf:type owl:NamedIndividual ,
                             eme:MacroPeriodKind ;
                    rdfs:comment "For the period defined by the start and end of the TimePeriod element in the message."@en .


#-- sr
eme:sr rdf:type owl:NamedIndividual ,
                eme:UnitSymbol ;
       rdfs:comment "Solid angle in steradians m2m2." ;
       rdfs:label "sr"@en .


#-- steam
eme:steam rdf:type owl:NamedIndividual ,
                   eme:CommodityKind ;
          rdfs:comment "Water in steam form, usually used for heating."@en .


#-- sum
eme:sum rdf:type owl:NamedIndividual ,
                 eme:AggregateKind ;
        rdfs:comment "The accumulated sum."@en .


#-- summation
eme:summation rdf:type owl:NamedIndividual ,
                       eme:AccumulationKind ;
              rdfs:comment """A form of accumulation which is selective with respect to time. 
Note : 'summation' could be considered a specialisation of 'bulkQuantity' as it selectively accumulates pulses over a timing pattern (while 'bulkQuantity' accumulates pulses all of the time)."""@en .


#-- swell
eme:swell rdf:type owl:NamedIndividual ,
                   eme:MeasurementKind ;
          rdfs:label "swell"@en .


#-- switchArmed
eme:switchArmed rdf:type owl:NamedIndividual ,
                         eme:MeasurementKind ;
                rdfs:label "switchArmed"@en .


#-- switchDisabled
eme:switchDisabled rdf:type owl:NamedIndividual ,
                            eme:MeasurementKind ;
                   rdfs:label "switchDisabled"@en .


#-- switchPosition
eme:switchPosition rdf:type owl:NamedIndividual ,
                            eme:MeasurementKind ;
                   rdfs:label "switchPosition"@en .


#-- tamper
eme:tamper rdf:type owl:NamedIndividual ,
                    eme:MeasurementKind ;
           rdfs:label "tamper"@en .


#-- tapPosition
eme:tapPosition rdf:type owl:NamedIndividual ,
                         eme:MeasurementKind ;
                rdfs:label "tapPosition"@en .


#-- tariffRate
eme:tariffRate rdf:type owl:NamedIndividual ,
                        eme:MeasurementKind ;
               rdfs:label "tariffRate"@en .


#-- temperature
eme:temperature rdf:type owl:NamedIndividual ,
                         eme:MeasurementKind ;
                rdfs:label "temperature"@en .


#-- tenMinute
eme:tenMinute rdf:type owl:NamedIndividual ,
                       eme:MeasuringPeriodKind ;
              rdfs:comment "10-minute"@en .


#-- therm
eme:therm rdf:type owl:NamedIndividual ,
                   eme:UnitSymbol ;
          rdfs:comment "Energy therms." ;
          rdfs:label "therm"@en .


#-- thirdMaximum
eme:thirdMaximum rdf:type owl:NamedIndividual ,
                          eme:AggregateKind ;
                 rdfs:comment "The third highest value observed."@en .


#-- thirtyMinute
eme:thirtyMinute rdf:type owl:NamedIndividual ,
                          eme:MeasuringPeriodKind ;
                 rdfs:comment "30-minute"@en .


#-- threeMinute
eme:threeMinute rdf:type owl:NamedIndividual ,
                         eme:MeasuringPeriodKind ;
                rdfs:comment "3-minute"@en .


#-- timeDelay
eme:timeDelay rdf:type owl:NamedIndividual ,
                       eme:AccumulationKind ;
              rdfs:comment "A form of computation which introduces a time delay characteristic to the data value."@en .


#-- tonne
eme:tonne rdf:type owl:NamedIndividual ,
                   eme:UnitSymbol ;
          rdfs:comment "Mass in tons tonne or metric  ton 1000 kg  1 Mg." ;
          rdfs:label "tonne"@en .


#-- total
eme:total rdf:type owl:NamedIndividual ,
                   eme:FlowDirectionKind ;
          rdfs:comment """|Forward| + |Reverse|, See 61968-2.
The sum of the commodity in all quadrants Q1+Q2+Q3+Q4.
In polyphase metering, the total energy register is incremented when the absolute value of the sum of the phase energies is greater than zero:
<img src=\"HTS_1.PNG\" width=\"217\" height=\"16\" border=\"0\" alt=\"graphic\"/>"""@en .


#-- totalByPhase
eme:totalByPhase rdf:type owl:NamedIndividual ,
                          eme:FlowDirectionKind ;
                 rdfs:comment """In polyphase metering, the total by phase energy register is incremented when the sum of the absolute values of the phase energies is greater than zero:
<img src=\"HTS_1.PNG\" width=\"234\" height=\"16\" border=\"0\" alt=\"graphic\"/>
In single phase metering, the formulas for “Total” and “Total by phase” collapse to the same expression. For communication purposes however, the “Total” enumeration should be used with single phase meter data."""@en .


#-- totalHarmonicDistortion
eme:totalHarmonicDistortion rdf:type owl:NamedIndividual ,
                                     eme:MeasurementKind ;
                            rdfs:label "totalHarmonicDistortion"@en .


#-- transformerLoss
eme:transformerLoss rdf:type owl:NamedIndividual ,
                             eme:MeasurementKind ;
                    rdfs:label "transformerLoss"@en .


#-- tvLicence
eme:tvLicence rdf:type owl:NamedIndividual ,
                       eme:CommodityKind ;
              rdfs:comment "Television"@en .


#-- twentyMinute
eme:twentyMinute rdf:type owl:NamedIndividual ,
                          eme:MeasuringPeriodKind ;
                 rdfs:comment "20-minute interval"@en .


#-- twentyfourHour
eme:twentyfourHour rdf:type owl:NamedIndividual ,
                            eme:MeasuringPeriodKind ;
                   rdfs:comment "24-hour"@en .


#-- twoMinute
eme:twoMinute rdf:type owl:NamedIndividual ,
                       eme:MeasuringPeriodKind ;
              rdfs:comment "2-minute"@en .


#-- twoWayAddress
eme:twoWayAddress rdf:type owl:NamedIndividual ,
                           eme:MeasurementKind ;
                  rdfs:label "twoWayAddress"@en .


#-- unipedeVoltageDip10to15
eme:unipedeVoltageDip10to15 rdf:type owl:NamedIndividual ,
                                     eme:MeasurementKind ;
                            rdfs:label "unipedeVoltageDip10to15"@en .


#-- unipedeVoltageDip15to30
eme:unipedeVoltageDip15to30 rdf:type owl:NamedIndividual ,
                                     eme:MeasurementKind ;
                            rdfs:label "unipedeVoltageDip15to30"@en .


#-- unipedeVoltageDip30to60
eme:unipedeVoltageDip30to60 rdf:type owl:NamedIndividual ,
                                     eme:MeasurementKind ;
                            rdfs:label "unipedeVoltageDip30to60"@en .


#-- unipedeVoltageDip60to90
eme:unipedeVoltageDip60to90 rdf:type owl:NamedIndividual ,
                                     eme:MeasurementKind ;
                            rdfs:label "unipedeVoltageDip60to90"@en .


#-- unipedeVoltageDip90to100
eme:unipedeVoltageDip90to100 rdf:type owl:NamedIndividual ,
                                      eme:MeasurementKind ;
                             rdfs:label "unipedeVoltageDip90to100"@en .


#-- voltage
eme:voltage rdf:type owl:NamedIndividual ,
                     eme:MeasurementKind ;
            rdfs:label "voltage"@en .


#-- voltageAngle
eme:voltageAngle rdf:type owl:NamedIndividual ,
                          eme:MeasurementKind ;
                 rdfs:label "voltageAngle"@en .


#-- voltageExcursion
eme:voltageExcursion rdf:type owl:NamedIndividual ,
                              eme:MeasurementKind ;
                     rdfs:label "voltageExcursion"@en .


#-- voltageImbalance
eme:voltageImbalance rdf:type owl:NamedIndividual ,
                              eme:MeasurementKind ;
                     rdfs:label "voltageImbalance"@en .


#-- volume
eme:volume rdf:type owl:NamedIndividual ,
                    eme:MeasurementKind ;
           rdfs:comment "Clarified  from Ed. 1. to indicate fluid volume" ;
           rdfs:label "volume"@en .


#-- volumetricFlow
eme:volumetricFlow rdf:type owl:NamedIndividual ,
                            eme:MeasurementKind ;
                   rdfs:label "volumetricFlow"@en .


#-- wasteWater
eme:wasteWater rdf:type owl:NamedIndividual ,
                        eme:CommodityKind ;
               rdfs:comment "(Sewerage)"@en .


#-- watchdogTimeout
eme:watchdogTimeout rdf:type owl:NamedIndividual ,
                             eme:MeasurementKind ;
                    rdfs:label "watchdogTimeout"@en .


#-- weekly
eme:weekly rdf:type owl:NamedIndividual ,
                    eme:MacroPeriodKind ;
           rdfs:comment "Weekly period starting at midnight on the first day of the week and ending the instant before midnight the last day of the week. If within the current week, it specifies the period from the start of the week until \"now.\""@en .


#-- windMachine
eme:windMachine rdf:type owl:NamedIndividual ,
                         eme:CustomerKind ;
                rdfs:comment "Wind machine customer."@en .


#-- y
eme:y rdf:type owl:NamedIndividual ,
               eme:UnitMultiplier ;
      rdfs:comment "Yocto 1024." ;
      rdfs:label "y"@en .


#-- z
eme:z rdf:type owl:NamedIndividual ,
               eme:UnitMultiplier ;
      rdfs:comment "Zepto 1021." ;
      rdfs:label "z"@en .


#-- zeroFlowDuration
eme:zeroFlowDuration rdf:type owl:NamedIndividual ,
                              eme:MeasurementKind ;
                     rdfs:label "zeroFlowDuration"@en .


#-- zeroSequence
eme:zeroSequence rdf:type owl:NamedIndividual ,
                          eme:MeasurementKind ;
                 rdfs:label "zeroSequence"@en .

